tests/IIR.bpl
@@ -1,25 +1,23 @@
 // ---------------------------------------------------------------
 // -- Types and global variables ---------------------------------
 // ---------------------------------------------------------------
-type Chan;
+type Ref;
+type Chan a;
 type Field a;
 type Actor;
-type CType = [Chan]int;
-type MType = <a>[Chan][int][Field a]a;
-type State;
+type CType = <a>[Chan a]int;
+type MType = <a>[Chan a][int]a;
+type Obj = <a>[Field a]a;
+type HType = [Ref]Obj;
 
 var M: MType;
 var C: CType;
 var R: CType;
 var I: CType;
 
+var H: HType;
+
 const unique this#: Actor;
-
-const unique data#int: Field int;
-const unique data#bool: Field bool;
-
-type List a = [int]a;
-var AT#intlst: List int;
 
 function AT#Min(x:int, y: int): int { if x <= y then x else y }
 
@@ -61,11 +59,11 @@ axiom (forall a: int :: (
 // ---------------------------------------------------------------
 
 procedure add#init#0()
-  modifies C, R, M, I;
+  modifies C, R, M, I, H;
 {
-  var in1: Chan;
-  var in2: Chan;
-  var out: Chan;
+  var in1: Chan (int);
+  var in2: Chan (int);
+  var out: Chan (int);
   assume (in1 != in2) && (in1 != out) && (in2 != out);
   assume R[in1] == 0;
   assume R[in2] == 0;
@@ -73,15 +71,15 @@ procedure add#init#0()
   assert {:msg "Initialization might not establish the invariant (#0)"} R[in1] == C[out];
   assert {:msg "Initialization might not establish the invariant (#1)"} R[in2] == C[out];
   assert {:msg "Initialization might not establish the invariant (#2)"} (forall idx$: int :: 
-    (0 <= idx$) && (idx$ < C[out]) ==> (M[out][idx$][data#int] == (M[in1][idx$][data#int] + M[in2][idx$][data#int]))
+    (0 <= idx$) && (idx$ < C[out]) ==> (M[out][idx$] == (M[in1][idx$] + M[in2][idx$]))
   );
 }
 procedure add#anon$0#1()
-  modifies C, R, M, I;
+  modifies C, R, M, I, H;
 {
-  var in1: Chan;
-  var in2: Chan;
-  var out: Chan;
+  var in1: Chan (int);
+  var in2: Chan (int);
+  var out: Chan (int);
   var in1#0: int;
   var in2#0: int;
   assume (in1 != in2) && (in1 != out) && (in2 != out);
@@ -91,81 +89,81 @@ procedure add#anon$0#1()
   assume R[in1] == C[out];
   assume R[in2] == C[out];
   assume (forall idx$: int :: 
-    (0 <= idx$) && (idx$ < C[out]) ==> (M[out][idx$][data#int] == (M[in1][idx$][data#int] + M[in2][idx$][data#int]))
+    (0 <= idx$) && (idx$ < C[out]) ==> (M[out][idx$] == (M[in1][idx$] + M[in2][idx$]))
   );
-  in1#0 := M[in1][R[in1]][data#int];
+  in1#0 := M[in1][R[in1]];
   R[in1] := R[in1] + 1;
-  in2#0 := M[in2][R[in2]][data#int];
+  in2#0 := M[in2][R[in2]];
   R[in2] := R[in2] + 1;
-  M[out][C[out]][data#int] := in1#0 + in2#0;
+  M[out][C[out]] := in1#0 + in2#0;
   C[out] := C[out] + 1;
   assert {:msg "Action at 2.3 might not preserve invariant (#3)"} R[in1] == C[out];
   assert {:msg "Action at 2.3 might not preserve invariant (#4)"} R[in2] == C[out];
   assert {:msg "Action at 2.3 might not preserve invariant (#5)"} (forall idx$: int :: 
-    (0 <= idx$) && (idx$ < C[out]) ==> (M[out][idx$][data#int] == (M[in1][idx$][data#int] + M[in2][idx$][data#int]))
+    (0 <= idx$) && (idx$ < C[out]) ==> (M[out][idx$] == (M[in1][idx$] + M[in2][idx$]))
   );
 }
 procedure delay#init#2()
-  modifies C, R, M, I;
+  modifies C, R, M, I, H;
 {
-  var in: Chan;
-  var out: Chan;
+  var in: Chan (int);
+  var out: Chan (int);
   var k: int;
   assume in != out;
   assume R[in] == 0;
   assume C[out] == 0;
-  M[out][C[out]][data#int] := k;
+  M[out][C[out]] := k;
   C[out] := C[out] + 1;
-  assert {:msg "6.20: Initialization might not establish the invariant (#6)"} M[out][0][data#int] == k;
+  assert {:msg "6.20: Initialization might not establish the invariant (#6)"} M[out][0] == k;
   assert {:msg "Initialization might not establish the invariant (#7)"} R[in] == (C[out] - 1);
   assert {:msg "Initialization might not establish the invariant (#8)"} (forall idx$: int :: 
-    (1 <= idx$) && (idx$ < C[out]) ==> (M[out][idx$][data#int] == M[in][idx$ - 1][data#int])
+    (1 <= idx$) && (idx$ < C[out]) ==> (M[out][idx$] == M[in][idx$ - 1])
   );
 }
 procedure delay#anon$2#3()
-  modifies C, R, M, I;
+  modifies C, R, M, I, H;
 {
-  var in: Chan;
-  var out: Chan;
+  var in: Chan (int);
+  var out: Chan (int);
   var k: int;
   var in#0: int;
   assume in != out;
   assume 0 <= R[in];
   assume 0 <= C[out];
-  assume M[out][0][data#int] == k;
+  assume M[out][0] == k;
   assume R[in] == (C[out] - 1);
   assume (forall idx$: int :: 
-    (1 <= idx$) && (idx$ < C[out]) ==> (M[out][idx$][data#int] == M[in][idx$ - 1][data#int])
+    (1 <= idx$) && (idx$ < C[out]) ==> (M[out][idx$] == M[in][idx$ - 1])
   );
-  in#0 := M[in][R[in]][data#int];
+  in#0 := M[in][R[in]];
   R[in] := R[in] + 1;
-  M[out][C[out]][data#int] := in#0;
+  M[out][C[out]] := in#0;
   C[out] := C[out] + 1;
-  assert {:msg "6.20: Action at 8.3 might not preserve invariant (#9)"} M[out][0][data#int] == k;
+  assert {:msg "6.20: Action at 8.3 might not preserve invariant (#9)"} M[out][0] == k;
   assert {:msg "Action at 8.3 might not preserve invariant (#10)"} R[in] == (C[out] - 1);
   assert {:msg "Action at 8.3 might not preserve invariant (#11)"} (forall idx$: int :: 
-    (1 <= idx$) && (idx$ < C[out]) ==> (M[out][idx$][data#int] == M[in][idx$ - 1][data#int])
+    (1 <= idx$) && (idx$ < C[out]) ==> (M[out][idx$] == M[in][idx$ - 1])
   );
 }
 procedure mulc#init#4()
-  modifies C, R, M, I;
+  modifies C, R, M, I, H;
 {
-  var in: Chan;
-  var out: Chan;
+  var in: Chan (int);
+  var out: Chan (int);
   var c: int;
   assume in != out;
   assume R[in] == 0;
   assume C[out] == 0;
   assert {:msg "Initialization might not establish the invariant (#12)"} R[in] == C[out];
   assert {:msg "Initialization might not establish the invariant (#13)"} (forall idx$: int :: 
-    (0 <= idx$) && (idx$ < C[out]) ==> (M[out][idx$][data#int] == (c * M[in][idx$][data#int]))
+    (0 <= idx$) && (idx$ < C[out]) ==> (M[out][idx$] == (c * M[in][idx$]))
   );
 }
 procedure mulc#anon$3#5()
-  modifies C, R, M, I;
+  modifies C, R, M, I, H;
 {
-  var in: Chan;
-  var out: Chan;
+  var in: Chan (int);
+  var out: Chan (int);
   var c: int;
   var in#0: int;
   assume in != out;
@@ -173,36 +171,36 @@ procedure mulc#anon$3#5()
   assume 0 <= C[out];
   assume R[in] == C[out];
   assume (forall idx$: int :: 
-    (0 <= idx$) && (idx$ < C[out]) ==> (M[out][idx$][data#int] == (c * M[in][idx$][data#int]))
+    (0 <= idx$) && (idx$ < C[out]) ==> (M[out][idx$] == (c * M[in][idx$]))
   );
-  in#0 := M[in][R[in]][data#int];
+  in#0 := M[in][R[in]];
   R[in] := R[in] + 1;
-  M[out][C[out]][data#int] := c * in#0;
+  M[out][C[out]] := c * in#0;
   C[out] := C[out] + 1;
   assert {:msg "Action at 12.3 might not preserve invariant (#14)"} R[in] == C[out];
   assert {:msg "Action at 12.3 might not preserve invariant (#15)"} (forall idx$: int :: 
-    (0 <= idx$) && (idx$ < C[out]) ==> (M[out][idx$][data#int] == (c * M[in][idx$][data#int]))
+    (0 <= idx$) && (idx$ < C[out]) ==> (M[out][idx$] == (c * M[in][idx$]))
   );
 }
 procedure rshift#init#6()
-  modifies C, R, M, I;
+  modifies C, R, M, I, H;
 {
-  var in: Chan;
-  var out: Chan;
+  var in: Chan (int);
+  var out: Chan (int);
   var s: int;
   assume in != out;
   assume R[in] == 0;
   assume C[out] == 0;
   assert {:msg "Initialization might not establish the invariant (#16)"} R[in] == C[out];
   assert {:msg "Initialization might not establish the invariant (#17)"} (forall idx$: int :: 
-    (0 <= idx$) && (idx$ < C[out]) ==> (M[out][idx$][data#int] == AT#RShift(M[in][idx$][data#int], s))
+    (0 <= idx$) && (idx$ < C[out]) ==> (M[out][idx$] == AT#RShift(M[in][idx$], s))
   );
 }
 procedure rshift#anon$4#7()
-  modifies C, R, M, I;
+  modifies C, R, M, I, H;
 {
-  var in: Chan;
-  var out: Chan;
+  var in: Chan (int);
+  var out: Chan (int);
   var s: int;
   var in#0: int;
   assume in != out;
@@ -210,23 +208,23 @@ procedure rshift#anon$4#7()
   assume 0 <= C[out];
   assume R[in] == C[out];
   assume (forall idx$: int :: 
-    (0 <= idx$) && (idx$ < C[out]) ==> (M[out][idx$][data#int] == AT#RShift(M[in][idx$][data#int], s))
+    (0 <= idx$) && (idx$ < C[out]) ==> (M[out][idx$] == AT#RShift(M[in][idx$], s))
   );
-  in#0 := M[in][R[in]][data#int];
+  in#0 := M[in][R[in]];
   R[in] := R[in] + 1;
-  M[out][C[out]][data#int] := AT#RShift(in#0, s);
+  M[out][C[out]] := AT#RShift(in#0, s);
   C[out] := C[out] + 1;
   assert {:msg "Action at 16.3 might not preserve invariant (#18)"} R[in] == C[out];
   assert {:msg "Action at 16.3 might not preserve invariant (#19)"} (forall idx$: int :: 
-    (0 <= idx$) && (idx$ < C[out]) ==> (M[out][idx$][data#int] == AT#RShift(M[in][idx$][data#int], s))
+    (0 <= idx$) && (idx$ < C[out]) ==> (M[out][idx$] == AT#RShift(M[in][idx$], s))
   );
 }
 procedure split#init#8()
-  modifies C, R, M, I;
+  modifies C, R, M, I, H;
 {
-  var in: Chan;
-  var out1: Chan;
-  var out2: Chan;
+  var in: Chan (int);
+  var out1: Chan (int);
+  var out2: Chan (int);
   assume (in != out1) && (in != out2) && (out1 != out2);
   assume R[in] == 0;
   assume C[out1] == 0;
@@ -234,18 +232,18 @@ procedure split#init#8()
   assert {:msg "Initialization might not establish the invariant (#20)"} R[in] == C[out1];
   assert {:msg "Initialization might not establish the invariant (#21)"} R[in] == C[out2];
   assert {:msg "Initialization might not establish the invariant (#22)"} (forall idx$: int :: 
-    (0 <= idx$) && (idx$ < C[out1]) ==> (M[out1][idx$][data#int] == M[in][idx$][data#int])
+    (0 <= idx$) && (idx$ < C[out1]) ==> (M[out1][idx$] == M[in][idx$])
   );
   assert {:msg "Initialization might not establish the invariant (#23)"} (forall idx$: int :: 
-    (0 <= idx$) && (idx$ < C[out2]) ==> (M[out2][idx$][data#int] == M[in][idx$][data#int])
+    (0 <= idx$) && (idx$ < C[out2]) ==> (M[out2][idx$] == M[in][idx$])
   );
 }
 procedure split#anon$5#9()
-  modifies C, R, M, I;
+  modifies C, R, M, I, H;
 {
-  var in: Chan;
-  var out1: Chan;
-  var out2: Chan;
+  var in: Chan (int);
+  var out1: Chan (int);
+  var out2: Chan (int);
   var in#0: int;
   assume (in != out1) && (in != out2) && (out1 != out2);
   assume 0 <= R[in];
@@ -254,28 +252,28 @@ procedure split#anon$5#9()
   assume R[in] == C[out1];
   assume R[in] == C[out2];
   assume (forall idx$: int :: 
-    (0 <= idx$) && (idx$ < C[out1]) ==> (M[out1][idx$][data#int] == M[in][idx$][data#int])
+    (0 <= idx$) && (idx$ < C[out1]) ==> (M[out1][idx$] == M[in][idx$])
   );
   assume (forall idx$: int :: 
-    (0 <= idx$) && (idx$ < C[out2]) ==> (M[out2][idx$][data#int] == M[in][idx$][data#int])
+    (0 <= idx$) && (idx$ < C[out2]) ==> (M[out2][idx$] == M[in][idx$])
   );
-  in#0 := M[in][R[in]][data#int];
+  in#0 := M[in][R[in]];
   R[in] := R[in] + 1;
-  M[out1][C[out1]][data#int] := in#0;
+  M[out1][C[out1]] := in#0;
   C[out1] := C[out1] + 1;
-  M[out2][C[out2]][data#int] := in#0;
+  M[out2][C[out2]] := in#0;
   C[out2] := C[out2] + 1;
   assert {:msg "Action at 20.3 might not preserve invariant (#24)"} R[in] == C[out1];
   assert {:msg "Action at 20.3 might not preserve invariant (#25)"} R[in] == C[out2];
   assert {:msg "Action at 20.3 might not preserve invariant (#26)"} (forall idx$: int :: 
-    (0 <= idx$) && (idx$ < C[out1]) ==> (M[out1][idx$][data#int] == M[in][idx$][data#int])
+    (0 <= idx$) && (idx$ < C[out1]) ==> (M[out1][idx$] == M[in][idx$])
   );
   assert {:msg "Action at 20.3 might not preserve invariant (#27)"} (forall idx$: int :: 
-    (0 <= idx$) && (idx$ < C[out2]) ==> (M[out2][idx$][data#int] == M[in][idx$][data#int])
+    (0 <= idx$) && (idx$ < C[out2]) ==> (M[out2][idx$] == M[in][idx$])
   );
 }
 procedure iir#init#10()
-  modifies C, R, M, I;
+  modifies C, R, M, I, H;
 {
   var iir#del1: Actor;
   var iir#mul1: Actor;
@@ -283,24 +281,16 @@ procedure iir#init#10()
   var iir#rsh1: Actor;
   var iir#add1: Actor;
   var iir#spl1: Actor;
-  var iir#a: Chan;
-  var iir#a#data: Field (int);
-  var iir#b: Chan;
-  var iir#b#data: Field (int);
-  var iir#c: Chan;
-  var iir#c#data: Field (int);
-  var iir#d: Chan;
-  var iir#d#data: Field (int);
-  var iir#e: Chan;
-  var iir#e#data: Field (int);
-  var iir#f: Chan;
-  var iir#f#data: Field (int);
-  var iir#g: Chan;
-  var iir#g#data: Field (int);
-  var iir#h: Chan;
-  var iir#h#data: Field (int);
+  var iir#a: Chan (int);
+  var iir#b: Chan (int);
+  var iir#c: Chan (int);
+  var iir#d: Chan (int);
+  var iir#e: Chan (int);
+  var iir#f: Chan (int);
+  var iir#g: Chan (int);
+  var iir#h: Chan (int);
   assume (iir#del1 != iir#mul1) && (iir#del1 != iir#mul2) && (iir#del1 != iir#rsh1) && (iir#del1 != iir#add1) && (iir#del1 != iir#spl1) && (iir#mul1 != iir#mul2) && (iir#mul1 != iir#rsh1) && (iir#mul1 != iir#add1) && (iir#mul1 != iir#spl1) && (iir#mul2 != iir#rsh1) && (iir#mul2 != iir#add1) && (iir#mul2 != iir#spl1) && (iir#rsh1 != iir#add1) && (iir#rsh1 != iir#spl1) && (iir#add1 != iir#spl1);
-  assume (iir#a != iir#b) && (iir#a != iir#c) && (iir#a != iir#d) && (iir#a != iir#e) && (iir#a != iir#f) && (iir#a != iir#g) && (iir#a != iir#h) && (iir#a#data != iir#b#data) && (iir#a#data != iir#c#data) && (iir#a#data != iir#d#data) && (iir#a#data != iir#e#data) && (iir#a#data != iir#f#data) && (iir#a#data != iir#g#data) && (iir#a#data != iir#h#data) && (iir#b != iir#c) && (iir#b != iir#d) && (iir#b != iir#e) && (iir#b != iir#f) && (iir#b != iir#g) && (iir#b != iir#h) && (iir#b#data != iir#c#data) && (iir#b#data != iir#d#data) && (iir#b#data != iir#e#data) && (iir#b#data != iir#f#data) && (iir#b#data != iir#g#data) && (iir#b#data != iir#h#data) && (iir#c != iir#d) && (iir#c != iir#e) && (iir#c != iir#f) && (iir#c != iir#g) && (iir#c != iir#h) && (iir#c#data != iir#d#data) && (iir#c#data != iir#e#data) && (iir#c#data != iir#f#data) && (iir#c#data != iir#g#data) && (iir#c#data != iir#h#data) && (iir#d != iir#e) && (iir#d != iir#f) && (iir#d != iir#g) && (iir#d != iir#h) && (iir#d#data != iir#e#data) && (iir#d#data != iir#f#data) && (iir#d#data != iir#g#data) && (iir#d#data != iir#h#data) && (iir#e != iir#f) && (iir#e != iir#g) && (iir#e != iir#h) && (iir#e#data != iir#f#data) && (iir#e#data != iir#g#data) && (iir#e#data != iir#h#data) && (iir#f != iir#g) && (iir#f != iir#h) && (iir#f#data != iir#g#data) && (iir#f#data != iir#h#data) && (iir#g != iir#h) && (iir#g#data != iir#h#data);
+  assume (iir#a != iir#b) && (iir#a != iir#c) && (iir#a != iir#d) && (iir#a != iir#e) && (iir#a != iir#f) && (iir#a != iir#g) && (iir#a != iir#h) && (iir#b != iir#c) && (iir#b != iir#d) && (iir#b != iir#e) && (iir#b != iir#f) && (iir#b != iir#g) && (iir#b != iir#h) && (iir#c != iir#d) && (iir#c != iir#e) && (iir#c != iir#f) && (iir#c != iir#g) && (iir#c != iir#h) && (iir#d != iir#e) && (iir#d != iir#f) && (iir#d != iir#g) && (iir#d != iir#h) && (iir#e != iir#f) && (iir#e != iir#g) && (iir#e != iir#h) && (iir#f != iir#g) && (iir#f != iir#h) && (iir#g != iir#h);
   assume 0 <= I[iir#a];
   assume I[iir#a] <= R[iir#a];
   assume R[iir#a] <= C[iir#a];
@@ -343,7 +333,7 @@ procedure iir#init#10()
   assume C[iir#h] == 0;
   assume R[iir#h] == 0;
   assume 0 == 0;
-  M[iir#f][C[iir#f]][data#int] := 0;
+  M[iir#f][C[iir#f]] := 0;
   C[iir#f] := C[iir#f] + 1;
   assume 85 == 85;
   assume 171 == 171;
@@ -367,7 +357,7 @@ procedure iir#init#10()
   assert {:msg "Initialization of network 'iir' might not establish the network invariant: Unread tokens might be left on channel h (#43)"} (C[iir#h] - R[iir#h]) == 0;
 }
 procedure iir##delay#anon$2#11()
-  modifies C, R, M, I;
+  modifies C, R, M, I, H;
 {
   var iir#del1: Actor;
   var iir#mul1: Actor;
@@ -375,25 +365,17 @@ procedure iir##delay#anon$2#11()
   var iir#rsh1: Actor;
   var iir#add1: Actor;
   var iir#spl1: Actor;
-  var iir#a: Chan;
-  var iir#a#data: Field (int);
-  var iir#b: Chan;
-  var iir#b#data: Field (int);
-  var iir#c: Chan;
-  var iir#c#data: Field (int);
-  var iir#d: Chan;
-  var iir#d#data: Field (int);
-  var iir#e: Chan;
-  var iir#e#data: Field (int);
-  var iir#f: Chan;
-  var iir#f#data: Field (int);
-  var iir#g: Chan;
-  var iir#g#data: Field (int);
-  var iir#h: Chan;
-  var iir#h#data: Field (int);
+  var iir#a: Chan (int);
+  var iir#b: Chan (int);
+  var iir#c: Chan (int);
+  var iir#d: Chan (int);
+  var iir#e: Chan (int);
+  var iir#f: Chan (int);
+  var iir#g: Chan (int);
+  var iir#h: Chan (int);
   var in#i: int;
   assume (iir#del1 != iir#mul1) && (iir#del1 != iir#mul2) && (iir#del1 != iir#rsh1) && (iir#del1 != iir#add1) && (iir#del1 != iir#spl1) && (iir#mul1 != iir#mul2) && (iir#mul1 != iir#rsh1) && (iir#mul1 != iir#add1) && (iir#mul1 != iir#spl1) && (iir#mul2 != iir#rsh1) && (iir#mul2 != iir#add1) && (iir#mul2 != iir#spl1) && (iir#rsh1 != iir#add1) && (iir#rsh1 != iir#spl1) && (iir#add1 != iir#spl1);
-  assume (iir#a != iir#b) && (iir#a != iir#c) && (iir#a != iir#d) && (iir#a != iir#e) && (iir#a != iir#f) && (iir#a != iir#g) && (iir#a != iir#h) && (iir#a#data != iir#b#data) && (iir#a#data != iir#c#data) && (iir#a#data != iir#d#data) && (iir#a#data != iir#e#data) && (iir#a#data != iir#f#data) && (iir#a#data != iir#g#data) && (iir#a#data != iir#h#data) && (iir#b != iir#c) && (iir#b != iir#d) && (iir#b != iir#e) && (iir#b != iir#f) && (iir#b != iir#g) && (iir#b != iir#h) && (iir#b#data != iir#c#data) && (iir#b#data != iir#d#data) && (iir#b#data != iir#e#data) && (iir#b#data != iir#f#data) && (iir#b#data != iir#g#data) && (iir#b#data != iir#h#data) && (iir#c != iir#d) && (iir#c != iir#e) && (iir#c != iir#f) && (iir#c != iir#g) && (iir#c != iir#h) && (iir#c#data != iir#d#data) && (iir#c#data != iir#e#data) && (iir#c#data != iir#f#data) && (iir#c#data != iir#g#data) && (iir#c#data != iir#h#data) && (iir#d != iir#e) && (iir#d != iir#f) && (iir#d != iir#g) && (iir#d != iir#h) && (iir#d#data != iir#e#data) && (iir#d#data != iir#f#data) && (iir#d#data != iir#g#data) && (iir#d#data != iir#h#data) && (iir#e != iir#f) && (iir#e != iir#g) && (iir#e != iir#h) && (iir#e#data != iir#f#data) && (iir#e#data != iir#g#data) && (iir#e#data != iir#h#data) && (iir#f != iir#g) && (iir#f != iir#h) && (iir#f#data != iir#g#data) && (iir#f#data != iir#h#data) && (iir#g != iir#h) && (iir#g#data != iir#h#data);
+  assume (iir#a != iir#b) && (iir#a != iir#c) && (iir#a != iir#d) && (iir#a != iir#e) && (iir#a != iir#f) && (iir#a != iir#g) && (iir#a != iir#h) && (iir#b != iir#c) && (iir#b != iir#d) && (iir#b != iir#e) && (iir#b != iir#f) && (iir#b != iir#g) && (iir#b != iir#h) && (iir#c != iir#d) && (iir#c != iir#e) && (iir#c != iir#f) && (iir#c != iir#g) && (iir#c != iir#h) && (iir#d != iir#e) && (iir#d != iir#f) && (iir#d != iir#g) && (iir#d != iir#h) && (iir#e != iir#f) && (iir#e != iir#g) && (iir#e != iir#h) && (iir#f != iir#g) && (iir#f != iir#h) && (iir#g != iir#h);
   assume 0 <= I[iir#a];
   assume I[iir#a] <= R[iir#a];
   assume R[iir#a] <= C[iir#a];
@@ -427,70 +409,70 @@ procedure iir##delay#anon$2#11()
   assume I[iir#c] == I[iir#f];
   assume I[iir#d] == I[iir#g];
   assume I[iir#h] == I[iir#g];
-  assume M[iir#f][0][data#int] == 0;
+  assume M[iir#f][0] == 0;
   assume R[iir#e] == (C[iir#f] - 1);
   assume (forall idx$: int :: 
-    (1 <= idx$) && (idx$ < C[iir#f]) ==> (M[iir#f][idx$][data#int] == M[iir#e][idx$ - 1][data#int])
+    (1 <= idx$) && (idx$ < C[iir#f]) ==> (M[iir#f][idx$] == M[iir#e][idx$ - 1])
   );
   assume R[iir#a] == C[iir#b];
   assume (forall idx$: int :: 
-    (0 <= idx$) && (idx$ < C[iir#b]) ==> (M[iir#b][idx$][data#int] == (85 * M[iir#a][idx$][data#int]))
+    (0 <= idx$) && (idx$ < C[iir#b]) ==> (M[iir#b][idx$] == (85 * M[iir#a][idx$]))
   );
   assume R[iir#d] == C[iir#e];
   assume (forall idx$: int :: 
-    (0 <= idx$) && (idx$ < C[iir#e]) ==> (M[iir#e][idx$][data#int] == (171 * M[iir#d][idx$][data#int]))
+    (0 <= idx$) && (idx$ < C[iir#e]) ==> (M[iir#e][idx$] == (171 * M[iir#d][idx$]))
   );
   assume R[iir#c] == C[iir#g];
   assume (forall idx$: int :: 
-    (0 <= idx$) && (idx$ < C[iir#g]) ==> (M[iir#g][idx$][data#int] == AT#RShift(M[iir#c][idx$][data#int], 8))
+    (0 <= idx$) && (idx$ < C[iir#g]) ==> (M[iir#g][idx$] == AT#RShift(M[iir#c][idx$], 8))
   );
   assume R[iir#b] == C[iir#c];
   assume R[iir#f] == C[iir#c];
   assume (forall idx$: int :: 
-    (0 <= idx$) && (idx$ < C[iir#c]) ==> (M[iir#c][idx$][data#int] == (M[iir#b][idx$][data#int] + M[iir#f][idx$][data#int]))
+    (0 <= idx$) && (idx$ < C[iir#c]) ==> (M[iir#c][idx$] == (M[iir#b][idx$] + M[iir#f][idx$]))
   );
   assume R[iir#g] == C[iir#d];
   assume R[iir#g] == C[iir#h];
   assume (forall idx$: int :: 
-    (0 <= idx$) && (idx$ < C[iir#d]) ==> (M[iir#d][idx$][data#int] == M[iir#g][idx$][data#int])
+    (0 <= idx$) && (idx$ < C[iir#d]) ==> (M[iir#d][idx$] == M[iir#g][idx$])
   );
   assume (forall idx$: int :: 
-    (0 <= idx$) && (idx$ < C[iir#h]) ==> (M[iir#h][idx$][data#int] == M[iir#g][idx$][data#int])
+    (0 <= idx$) && (idx$ < C[iir#h]) ==> (M[iir#h][idx$] == M[iir#g][idx$])
   );
   assume 1 <= (C[iir#e] - R[iir#e]);
-  in#i := M[iir#e][R[iir#e]][data#int];
+  in#i := M[iir#e][R[iir#e]];
   R[iir#e] := R[iir#e] + 1;
-  M[iir#f][C[iir#f]][data#int] := in#i;
+  M[iir#f][C[iir#f]] := in#i;
   C[iir#f] := C[iir#f] + 1;
-  assume M[iir#f][0][data#int] == 0;
+  assume M[iir#f][0] == 0;
   assume R[iir#e] == (C[iir#f] - 1);
   assume (forall idx$: int :: 
-    (1 <= idx$) && (idx$ < C[iir#f]) ==> (M[iir#f][idx$][data#int] == M[iir#e][idx$ - 1][data#int])
+    (1 <= idx$) && (idx$ < C[iir#f]) ==> (M[iir#f][idx$] == M[iir#e][idx$ - 1])
   );
   assume R[iir#a] == C[iir#b];
   assume (forall idx$: int :: 
-    (0 <= idx$) && (idx$ < C[iir#b]) ==> (M[iir#b][idx$][data#int] == (85 * M[iir#a][idx$][data#int]))
+    (0 <= idx$) && (idx$ < C[iir#b]) ==> (M[iir#b][idx$] == (85 * M[iir#a][idx$]))
   );
   assume R[iir#d] == C[iir#e];
   assume (forall idx$: int :: 
-    (0 <= idx$) && (idx$ < C[iir#e]) ==> (M[iir#e][idx$][data#int] == (171 * M[iir#d][idx$][data#int]))
+    (0 <= idx$) && (idx$ < C[iir#e]) ==> (M[iir#e][idx$] == (171 * M[iir#d][idx$]))
   );
   assume R[iir#c] == C[iir#g];
   assume (forall idx$: int :: 
-    (0 <= idx$) && (idx$ < C[iir#g]) ==> (M[iir#g][idx$][data#int] == AT#RShift(M[iir#c][idx$][data#int], 8))
+    (0 <= idx$) && (idx$ < C[iir#g]) ==> (M[iir#g][idx$] == AT#RShift(M[iir#c][idx$], 8))
   );
   assume R[iir#b] == C[iir#c];
   assume R[iir#f] == C[iir#c];
   assume (forall idx$: int :: 
-    (0 <= idx$) && (idx$ < C[iir#c]) ==> (M[iir#c][idx$][data#int] == (M[iir#b][idx$][data#int] + M[iir#f][idx$][data#int]))
+    (0 <= idx$) && (idx$ < C[iir#c]) ==> (M[iir#c][idx$] == (M[iir#b][idx$] + M[iir#f][idx$]))
   );
   assume R[iir#g] == C[iir#d];
   assume R[iir#g] == C[iir#h];
   assume (forall idx$: int :: 
-    (0 <= idx$) && (idx$ < C[iir#d]) ==> (M[iir#d][idx$][data#int] == M[iir#g][idx$][data#int])
+    (0 <= idx$) && (idx$ < C[iir#d]) ==> (M[iir#d][idx$] == M[iir#g][idx$])
   );
   assume (forall idx$: int :: 
-    (0 <= idx$) && (idx$ < C[iir#h]) ==> (M[iir#h][idx$][data#int] == M[iir#g][idx$][data#int])
+    (0 <= idx$) && (idx$ < C[iir#h]) ==> (M[iir#h][idx$] == M[iir#g][idx$])
   );
   assert {:msg "Action at 8.3 ('anon$2') for actor instance 'del1' might not preserve the channel invariant (#44)"} I[iir#f] == I[iir#e];
   assert {:msg "Action at 8.3 ('anon$2') for actor instance 'del1' might not preserve the channel invariant (#45)"} I[iir#b] == I[iir#a];
@@ -502,7 +484,7 @@ procedure iir##delay#anon$2#11()
   assert {:msg "Action at 8.3 ('anon$2') for actor instance 'del1' might not preserve the channel invariant (#51)"} I[iir#h] == I[iir#g];
 }
 procedure iir##mulc#anon$3#12()
-  modifies C, R, M, I;
+  modifies C, R, M, I, H;
 {
   var iir#del1: Actor;
   var iir#mul1: Actor;
@@ -510,25 +492,17 @@ procedure iir##mulc#anon$3#12()
   var iir#rsh1: Actor;
   var iir#add1: Actor;
   var iir#spl1: Actor;
-  var iir#a: Chan;
-  var iir#a#data: Field (int);
-  var iir#b: Chan;
-  var iir#b#data: Field (int);
-  var iir#c: Chan;
-  var iir#c#data: Field (int);
-  var iir#d: Chan;
-  var iir#d#data: Field (int);
-  var iir#e: Chan;
-  var iir#e#data: Field (int);
-  var iir#f: Chan;
-  var iir#f#data: Field (int);
-  var iir#g: Chan;
-  var iir#g#data: Field (int);
-  var iir#h: Chan;
-  var iir#h#data: Field (int);
+  var iir#a: Chan (int);
+  var iir#b: Chan (int);
+  var iir#c: Chan (int);
+  var iir#d: Chan (int);
+  var iir#e: Chan (int);
+  var iir#f: Chan (int);
+  var iir#g: Chan (int);
+  var iir#h: Chan (int);
   var in#i: int;
   assume (iir#del1 != iir#mul1) && (iir#del1 != iir#mul2) && (iir#del1 != iir#rsh1) && (iir#del1 != iir#add1) && (iir#del1 != iir#spl1) && (iir#mul1 != iir#mul2) && (iir#mul1 != iir#rsh1) && (iir#mul1 != iir#add1) && (iir#mul1 != iir#spl1) && (iir#mul2 != iir#rsh1) && (iir#mul2 != iir#add1) && (iir#mul2 != iir#spl1) && (iir#rsh1 != iir#add1) && (iir#rsh1 != iir#spl1) && (iir#add1 != iir#spl1);
-  assume (iir#a != iir#b) && (iir#a != iir#c) && (iir#a != iir#d) && (iir#a != iir#e) && (iir#a != iir#f) && (iir#a != iir#g) && (iir#a != iir#h) && (iir#a#data != iir#b#data) && (iir#a#data != iir#c#data) && (iir#a#data != iir#d#data) && (iir#a#data != iir#e#data) && (iir#a#data != iir#f#data) && (iir#a#data != iir#g#data) && (iir#a#data != iir#h#data) && (iir#b != iir#c) && (iir#b != iir#d) && (iir#b != iir#e) && (iir#b != iir#f) && (iir#b != iir#g) && (iir#b != iir#h) && (iir#b#data != iir#c#data) && (iir#b#data != iir#d#data) && (iir#b#data != iir#e#data) && (iir#b#data != iir#f#data) && (iir#b#data != iir#g#data) && (iir#b#data != iir#h#data) && (iir#c != iir#d) && (iir#c != iir#e) && (iir#c != iir#f) && (iir#c != iir#g) && (iir#c != iir#h) && (iir#c#data != iir#d#data) && (iir#c#data != iir#e#data) && (iir#c#data != iir#f#data) && (iir#c#data != iir#g#data) && (iir#c#data != iir#h#data) && (iir#d != iir#e) && (iir#d != iir#f) && (iir#d != iir#g) && (iir#d != iir#h) && (iir#d#data != iir#e#data) && (iir#d#data != iir#f#data) && (iir#d#data != iir#g#data) && (iir#d#data != iir#h#data) && (iir#e != iir#f) && (iir#e != iir#g) && (iir#e != iir#h) && (iir#e#data != iir#f#data) && (iir#e#data != iir#g#data) && (iir#e#data != iir#h#data) && (iir#f != iir#g) && (iir#f != iir#h) && (iir#f#data != iir#g#data) && (iir#f#data != iir#h#data) && (iir#g != iir#h) && (iir#g#data != iir#h#data);
+  assume (iir#a != iir#b) && (iir#a != iir#c) && (iir#a != iir#d) && (iir#a != iir#e) && (iir#a != iir#f) && (iir#a != iir#g) && (iir#a != iir#h) && (iir#b != iir#c) && (iir#b != iir#d) && (iir#b != iir#e) && (iir#b != iir#f) && (iir#b != iir#g) && (iir#b != iir#h) && (iir#c != iir#d) && (iir#c != iir#e) && (iir#c != iir#f) && (iir#c != iir#g) && (iir#c != iir#h) && (iir#d != iir#e) && (iir#d != iir#f) && (iir#d != iir#g) && (iir#d != iir#h) && (iir#e != iir#f) && (iir#e != iir#g) && (iir#e != iir#h) && (iir#f != iir#g) && (iir#f != iir#h) && (iir#g != iir#h);
   assume 0 <= I[iir#a];
   assume I[iir#a] <= R[iir#a];
   assume R[iir#a] <= C[iir#a];
@@ -562,70 +536,70 @@ procedure iir##mulc#anon$3#12()
   assume I[iir#c] == I[iir#f];
   assume I[iir#d] == I[iir#g];
   assume I[iir#h] == I[iir#g];
-  assume M[iir#f][0][data#int] == 0;
+  assume M[iir#f][0] == 0;
   assume R[iir#e] == (C[iir#f] - 1);
   assume (forall idx$: int :: 
-    (1 <= idx$) && (idx$ < C[iir#f]) ==> (M[iir#f][idx$][data#int] == M[iir#e][idx$ - 1][data#int])
+    (1 <= idx$) && (idx$ < C[iir#f]) ==> (M[iir#f][idx$] == M[iir#e][idx$ - 1])
   );
   assume R[iir#a] == C[iir#b];
   assume (forall idx$: int :: 
-    (0 <= idx$) && (idx$ < C[iir#b]) ==> (M[iir#b][idx$][data#int] == (85 * M[iir#a][idx$][data#int]))
+    (0 <= idx$) && (idx$ < C[iir#b]) ==> (M[iir#b][idx$] == (85 * M[iir#a][idx$]))
   );
   assume R[iir#d] == C[iir#e];
   assume (forall idx$: int :: 
-    (0 <= idx$) && (idx$ < C[iir#e]) ==> (M[iir#e][idx$][data#int] == (171 * M[iir#d][idx$][data#int]))
+    (0 <= idx$) && (idx$ < C[iir#e]) ==> (M[iir#e][idx$] == (171 * M[iir#d][idx$]))
   );
   assume R[iir#c] == C[iir#g];
   assume (forall idx$: int :: 
-    (0 <= idx$) && (idx$ < C[iir#g]) ==> (M[iir#g][idx$][data#int] == AT#RShift(M[iir#c][idx$][data#int], 8))
+    (0 <= idx$) && (idx$ < C[iir#g]) ==> (M[iir#g][idx$] == AT#RShift(M[iir#c][idx$], 8))
   );
   assume R[iir#b] == C[iir#c];
   assume R[iir#f] == C[iir#c];
   assume (forall idx$: int :: 
-    (0 <= idx$) && (idx$ < C[iir#c]) ==> (M[iir#c][idx$][data#int] == (M[iir#b][idx$][data#int] + M[iir#f][idx$][data#int]))
+    (0 <= idx$) && (idx$ < C[iir#c]) ==> (M[iir#c][idx$] == (M[iir#b][idx$] + M[iir#f][idx$]))
   );
   assume R[iir#g] == C[iir#d];
   assume R[iir#g] == C[iir#h];
   assume (forall idx$: int :: 
-    (0 <= idx$) && (idx$ < C[iir#d]) ==> (M[iir#d][idx$][data#int] == M[iir#g][idx$][data#int])
+    (0 <= idx$) && (idx$ < C[iir#d]) ==> (M[iir#d][idx$] == M[iir#g][idx$])
   );
   assume (forall idx$: int :: 
-    (0 <= idx$) && (idx$ < C[iir#h]) ==> (M[iir#h][idx$][data#int] == M[iir#g][idx$][data#int])
+    (0 <= idx$) && (idx$ < C[iir#h]) ==> (M[iir#h][idx$] == M[iir#g][idx$])
   );
   assume 1 <= (C[iir#a] - R[iir#a]);
-  in#i := M[iir#a][R[iir#a]][data#int];
+  in#i := M[iir#a][R[iir#a]];
   R[iir#a] := R[iir#a] + 1;
-  M[iir#b][C[iir#b]][data#int] := 85 * in#i;
+  M[iir#b][C[iir#b]] := 85 * in#i;
   C[iir#b] := C[iir#b] + 1;
-  assume M[iir#f][0][data#int] == 0;
+  assume M[iir#f][0] == 0;
   assume R[iir#e] == (C[iir#f] - 1);
   assume (forall idx$: int :: 
-    (1 <= idx$) && (idx$ < C[iir#f]) ==> (M[iir#f][idx$][data#int] == M[iir#e][idx$ - 1][data#int])
+    (1 <= idx$) && (idx$ < C[iir#f]) ==> (M[iir#f][idx$] == M[iir#e][idx$ - 1])
   );
   assume R[iir#a] == C[iir#b];
   assume (forall idx$: int :: 
-    (0 <= idx$) && (idx$ < C[iir#b]) ==> (M[iir#b][idx$][data#int] == (85 * M[iir#a][idx$][data#int]))
+    (0 <= idx$) && (idx$ < C[iir#b]) ==> (M[iir#b][idx$] == (85 * M[iir#a][idx$]))
   );
   assume R[iir#d] == C[iir#e];
   assume (forall idx$: int :: 
-    (0 <= idx$) && (idx$ < C[iir#e]) ==> (M[iir#e][idx$][data#int] == (171 * M[iir#d][idx$][data#int]))
+    (0 <= idx$) && (idx$ < C[iir#e]) ==> (M[iir#e][idx$] == (171 * M[iir#d][idx$]))
   );
   assume R[iir#c] == C[iir#g];
   assume (forall idx$: int :: 
-    (0 <= idx$) && (idx$ < C[iir#g]) ==> (M[iir#g][idx$][data#int] == AT#RShift(M[iir#c][idx$][data#int], 8))
+    (0 <= idx$) && (idx$ < C[iir#g]) ==> (M[iir#g][idx$] == AT#RShift(M[iir#c][idx$], 8))
   );
   assume R[iir#b] == C[iir#c];
   assume R[iir#f] == C[iir#c];
   assume (forall idx$: int :: 
-    (0 <= idx$) && (idx$ < C[iir#c]) ==> (M[iir#c][idx$][data#int] == (M[iir#b][idx$][data#int] + M[iir#f][idx$][data#int]))
+    (0 <= idx$) && (idx$ < C[iir#c]) ==> (M[iir#c][idx$] == (M[iir#b][idx$] + M[iir#f][idx$]))
   );
   assume R[iir#g] == C[iir#d];
   assume R[iir#g] == C[iir#h];
   assume (forall idx$: int :: 
-    (0 <= idx$) && (idx$ < C[iir#d]) ==> (M[iir#d][idx$][data#int] == M[iir#g][idx$][data#int])
+    (0 <= idx$) && (idx$ < C[iir#d]) ==> (M[iir#d][idx$] == M[iir#g][idx$])
   );
   assume (forall idx$: int :: 
-    (0 <= idx$) && (idx$ < C[iir#h]) ==> (M[iir#h][idx$][data#int] == M[iir#g][idx$][data#int])
+    (0 <= idx$) && (idx$ < C[iir#h]) ==> (M[iir#h][idx$] == M[iir#g][idx$])
   );
   assert {:msg "Action at 12.3 ('anon$3') for actor instance 'mul1' might not preserve the channel invariant (#52)"} I[iir#f] == I[iir#e];
   assert {:msg "Action at 12.3 ('anon$3') for actor instance 'mul1' might not preserve the channel invariant (#53)"} I[iir#b] == I[iir#a];
@@ -637,7 +611,7 @@ procedure iir##mulc#anon$3#12()
   assert {:msg "Action at 12.3 ('anon$3') for actor instance 'mul1' might not preserve the channel invariant (#59)"} I[iir#h] == I[iir#g];
 }
 procedure iir##mulc#anon$3#13()
-  modifies C, R, M, I;
+  modifies C, R, M, I, H;
 {
   var iir#del1: Actor;
   var iir#mul1: Actor;
@@ -645,25 +619,17 @@ procedure iir##mulc#anon$3#13()
   var iir#rsh1: Actor;
   var iir#add1: Actor;
   var iir#spl1: Actor;
-  var iir#a: Chan;
-  var iir#a#data: Field (int);
-  var iir#b: Chan;
-  var iir#b#data: Field (int);
-  var iir#c: Chan;
-  var iir#c#data: Field (int);
-  var iir#d: Chan;
-  var iir#d#data: Field (int);
-  var iir#e: Chan;
-  var iir#e#data: Field (int);
-  var iir#f: Chan;
-  var iir#f#data: Field (int);
-  var iir#g: Chan;
-  var iir#g#data: Field (int);
-  var iir#h: Chan;
-  var iir#h#data: Field (int);
+  var iir#a: Chan (int);
+  var iir#b: Chan (int);
+  var iir#c: Chan (int);
+  var iir#d: Chan (int);
+  var iir#e: Chan (int);
+  var iir#f: Chan (int);
+  var iir#g: Chan (int);
+  var iir#h: Chan (int);
   var in#i: int;
   assume (iir#del1 != iir#mul1) && (iir#del1 != iir#mul2) && (iir#del1 != iir#rsh1) && (iir#del1 != iir#add1) && (iir#del1 != iir#spl1) && (iir#mul1 != iir#mul2) && (iir#mul1 != iir#rsh1) && (iir#mul1 != iir#add1) && (iir#mul1 != iir#spl1) && (iir#mul2 != iir#rsh1) && (iir#mul2 != iir#add1) && (iir#mul2 != iir#spl1) && (iir#rsh1 != iir#add1) && (iir#rsh1 != iir#spl1) && (iir#add1 != iir#spl1);
-  assume (iir#a != iir#b) && (iir#a != iir#c) && (iir#a != iir#d) && (iir#a != iir#e) && (iir#a != iir#f) && (iir#a != iir#g) && (iir#a != iir#h) && (iir#a#data != iir#b#data) && (iir#a#data != iir#c#data) && (iir#a#data != iir#d#data) && (iir#a#data != iir#e#data) && (iir#a#data != iir#f#data) && (iir#a#data != iir#g#data) && (iir#a#data != iir#h#data) && (iir#b != iir#c) && (iir#b != iir#d) && (iir#b != iir#e) && (iir#b != iir#f) && (iir#b != iir#g) && (iir#b != iir#h) && (iir#b#data != iir#c#data) && (iir#b#data != iir#d#data) && (iir#b#data != iir#e#data) && (iir#b#data != iir#f#data) && (iir#b#data != iir#g#data) && (iir#b#data != iir#h#data) && (iir#c != iir#d) && (iir#c != iir#e) && (iir#c != iir#f) && (iir#c != iir#g) && (iir#c != iir#h) && (iir#c#data != iir#d#data) && (iir#c#data != iir#e#data) && (iir#c#data != iir#f#data) && (iir#c#data != iir#g#data) && (iir#c#data != iir#h#data) && (iir#d != iir#e) && (iir#d != iir#f) && (iir#d != iir#g) && (iir#d != iir#h) && (iir#d#data != iir#e#data) && (iir#d#data != iir#f#data) && (iir#d#data != iir#g#data) && (iir#d#data != iir#h#data) && (iir#e != iir#f) && (iir#e != iir#g) && (iir#e != iir#h) && (iir#e#data != iir#f#data) && (iir#e#data != iir#g#data) && (iir#e#data != iir#h#data) && (iir#f != iir#g) && (iir#f != iir#h) && (iir#f#data != iir#g#data) && (iir#f#data != iir#h#data) && (iir#g != iir#h) && (iir#g#data != iir#h#data);
+  assume (iir#a != iir#b) && (iir#a != iir#c) && (iir#a != iir#d) && (iir#a != iir#e) && (iir#a != iir#f) && (iir#a != iir#g) && (iir#a != iir#h) && (iir#b != iir#c) && (iir#b != iir#d) && (iir#b != iir#e) && (iir#b != iir#f) && (iir#b != iir#g) && (iir#b != iir#h) && (iir#c != iir#d) && (iir#c != iir#e) && (iir#c != iir#f) && (iir#c != iir#g) && (iir#c != iir#h) && (iir#d != iir#e) && (iir#d != iir#f) && (iir#d != iir#g) && (iir#d != iir#h) && (iir#e != iir#f) && (iir#e != iir#g) && (iir#e != iir#h) && (iir#f != iir#g) && (iir#f != iir#h) && (iir#g != iir#h);
   assume 0 <= I[iir#a];
   assume I[iir#a] <= R[iir#a];
   assume R[iir#a] <= C[iir#a];
@@ -697,70 +663,70 @@ procedure iir##mulc#anon$3#13()
   assume I[iir#c] == I[iir#f];
   assume I[iir#d] == I[iir#g];
   assume I[iir#h] == I[iir#g];
-  assume M[iir#f][0][data#int] == 0;
+  assume M[iir#f][0] == 0;
   assume R[iir#e] == (C[iir#f] - 1);
   assume (forall idx$: int :: 
-    (1 <= idx$) && (idx$ < C[iir#f]) ==> (M[iir#f][idx$][data#int] == M[iir#e][idx$ - 1][data#int])
+    (1 <= idx$) && (idx$ < C[iir#f]) ==> (M[iir#f][idx$] == M[iir#e][idx$ - 1])
   );
   assume R[iir#a] == C[iir#b];
   assume (forall idx$: int :: 
-    (0 <= idx$) && (idx$ < C[iir#b]) ==> (M[iir#b][idx$][data#int] == (85 * M[iir#a][idx$][data#int]))
+    (0 <= idx$) && (idx$ < C[iir#b]) ==> (M[iir#b][idx$] == (85 * M[iir#a][idx$]))
   );
   assume R[iir#d] == C[iir#e];
   assume (forall idx$: int :: 
-    (0 <= idx$) && (idx$ < C[iir#e]) ==> (M[iir#e][idx$][data#int] == (171 * M[iir#d][idx$][data#int]))
+    (0 <= idx$) && (idx$ < C[iir#e]) ==> (M[iir#e][idx$] == (171 * M[iir#d][idx$]))
   );
   assume R[iir#c] == C[iir#g];
   assume (forall idx$: int :: 
-    (0 <= idx$) && (idx$ < C[iir#g]) ==> (M[iir#g][idx$][data#int] == AT#RShift(M[iir#c][idx$][data#int], 8))
+    (0 <= idx$) && (idx$ < C[iir#g]) ==> (M[iir#g][idx$] == AT#RShift(M[iir#c][idx$], 8))
   );
   assume R[iir#b] == C[iir#c];
   assume R[iir#f] == C[iir#c];
   assume (forall idx$: int :: 
-    (0 <= idx$) && (idx$ < C[iir#c]) ==> (M[iir#c][idx$][data#int] == (M[iir#b][idx$][data#int] + M[iir#f][idx$][data#int]))
+    (0 <= idx$) && (idx$ < C[iir#c]) ==> (M[iir#c][idx$] == (M[iir#b][idx$] + M[iir#f][idx$]))
   );
   assume R[iir#g] == C[iir#d];
   assume R[iir#g] == C[iir#h];
   assume (forall idx$: int :: 
-    (0 <= idx$) && (idx$ < C[iir#d]) ==> (M[iir#d][idx$][data#int] == M[iir#g][idx$][data#int])
+    (0 <= idx$) && (idx$ < C[iir#d]) ==> (M[iir#d][idx$] == M[iir#g][idx$])
   );
   assume (forall idx$: int :: 
-    (0 <= idx$) && (idx$ < C[iir#h]) ==> (M[iir#h][idx$][data#int] == M[iir#g][idx$][data#int])
+    (0 <= idx$) && (idx$ < C[iir#h]) ==> (M[iir#h][idx$] == M[iir#g][idx$])
   );
   assume 1 <= (C[iir#d] - R[iir#d]);
-  in#i := M[iir#d][R[iir#d]][data#int];
+  in#i := M[iir#d][R[iir#d]];
   R[iir#d] := R[iir#d] + 1;
-  M[iir#e][C[iir#e]][data#int] := 171 * in#i;
+  M[iir#e][C[iir#e]] := 171 * in#i;
   C[iir#e] := C[iir#e] + 1;
-  assume M[iir#f][0][data#int] == 0;
+  assume M[iir#f][0] == 0;
   assume R[iir#e] == (C[iir#f] - 1);
   assume (forall idx$: int :: 
-    (1 <= idx$) && (idx$ < C[iir#f]) ==> (M[iir#f][idx$][data#int] == M[iir#e][idx$ - 1][data#int])
+    (1 <= idx$) && (idx$ < C[iir#f]) ==> (M[iir#f][idx$] == M[iir#e][idx$ - 1])
   );
   assume R[iir#a] == C[iir#b];
   assume (forall idx$: int :: 
-    (0 <= idx$) && (idx$ < C[iir#b]) ==> (M[iir#b][idx$][data#int] == (85 * M[iir#a][idx$][data#int]))
+    (0 <= idx$) && (idx$ < C[iir#b]) ==> (M[iir#b][idx$] == (85 * M[iir#a][idx$]))
   );
   assume R[iir#d] == C[iir#e];
   assume (forall idx$: int :: 
-    (0 <= idx$) && (idx$ < C[iir#e]) ==> (M[iir#e][idx$][data#int] == (171 * M[iir#d][idx$][data#int]))
+    (0 <= idx$) && (idx$ < C[iir#e]) ==> (M[iir#e][idx$] == (171 * M[iir#d][idx$]))
   );
   assume R[iir#c] == C[iir#g];
   assume (forall idx$: int :: 
-    (0 <= idx$) && (idx$ < C[iir#g]) ==> (M[iir#g][idx$][data#int] == AT#RShift(M[iir#c][idx$][data#int], 8))
+    (0 <= idx$) && (idx$ < C[iir#g]) ==> (M[iir#g][idx$] == AT#RShift(M[iir#c][idx$], 8))
   );
   assume R[iir#b] == C[iir#c];
   assume R[iir#f] == C[iir#c];
   assume (forall idx$: int :: 
-    (0 <= idx$) && (idx$ < C[iir#c]) ==> (M[iir#c][idx$][data#int] == (M[iir#b][idx$][data#int] + M[iir#f][idx$][data#int]))
+    (0 <= idx$) && (idx$ < C[iir#c]) ==> (M[iir#c][idx$] == (M[iir#b][idx$] + M[iir#f][idx$]))
   );
   assume R[iir#g] == C[iir#d];
   assume R[iir#g] == C[iir#h];
   assume (forall idx$: int :: 
-    (0 <= idx$) && (idx$ < C[iir#d]) ==> (M[iir#d][idx$][data#int] == M[iir#g][idx$][data#int])
+    (0 <= idx$) && (idx$ < C[iir#d]) ==> (M[iir#d][idx$] == M[iir#g][idx$])
   );
   assume (forall idx$: int :: 
-    (0 <= idx$) && (idx$ < C[iir#h]) ==> (M[iir#h][idx$][data#int] == M[iir#g][idx$][data#int])
+    (0 <= idx$) && (idx$ < C[iir#h]) ==> (M[iir#h][idx$] == M[iir#g][idx$])
   );
   assert {:msg "Action at 12.3 ('anon$3') for actor instance 'mul2' might not preserve the channel invariant (#60)"} I[iir#f] == I[iir#e];
   assert {:msg "Action at 12.3 ('anon$3') for actor instance 'mul2' might not preserve the channel invariant (#61)"} I[iir#b] == I[iir#a];
@@ -772,7 +738,7 @@ procedure iir##mulc#anon$3#13()
   assert {:msg "Action at 12.3 ('anon$3') for actor instance 'mul2' might not preserve the channel invariant (#67)"} I[iir#h] == I[iir#g];
 }
 procedure iir##rshift#anon$4#14()
-  modifies C, R, M, I;
+  modifies C, R, M, I, H;
 {
   var iir#del1: Actor;
   var iir#mul1: Actor;
@@ -780,25 +746,17 @@ procedure iir##rshift#anon$4#14()
   var iir#rsh1: Actor;
   var iir#add1: Actor;
   var iir#spl1: Actor;
-  var iir#a: Chan;
-  var iir#a#data: Field (int);
-  var iir#b: Chan;
-  var iir#b#data: Field (int);
-  var iir#c: Chan;
-  var iir#c#data: Field (int);
-  var iir#d: Chan;
-  var iir#d#data: Field (int);
-  var iir#e: Chan;
-  var iir#e#data: Field (int);
-  var iir#f: Chan;
-  var iir#f#data: Field (int);
-  var iir#g: Chan;
-  var iir#g#data: Field (int);
-  var iir#h: Chan;
-  var iir#h#data: Field (int);
+  var iir#a: Chan (int);
+  var iir#b: Chan (int);
+  var iir#c: Chan (int);
+  var iir#d: Chan (int);
+  var iir#e: Chan (int);
+  var iir#f: Chan (int);
+  var iir#g: Chan (int);
+  var iir#h: Chan (int);
   var in#i: int;
   assume (iir#del1 != iir#mul1) && (iir#del1 != iir#mul2) && (iir#del1 != iir#rsh1) && (iir#del1 != iir#add1) && (iir#del1 != iir#spl1) && (iir#mul1 != iir#mul2) && (iir#mul1 != iir#rsh1) && (iir#mul1 != iir#add1) && (iir#mul1 != iir#spl1) && (iir#mul2 != iir#rsh1) && (iir#mul2 != iir#add1) && (iir#mul2 != iir#spl1) && (iir#rsh1 != iir#add1) && (iir#rsh1 != iir#spl1) && (iir#add1 != iir#spl1);
-  assume (iir#a != iir#b) && (iir#a != iir#c) && (iir#a != iir#d) && (iir#a != iir#e) && (iir#a != iir#f) && (iir#a != iir#g) && (iir#a != iir#h) && (iir#a#data != iir#b#data) && (iir#a#data != iir#c#data) && (iir#a#data != iir#d#data) && (iir#a#data != iir#e#data) && (iir#a#data != iir#f#data) && (iir#a#data != iir#g#data) && (iir#a#data != iir#h#data) && (iir#b != iir#c) && (iir#b != iir#d) && (iir#b != iir#e) && (iir#b != iir#f) && (iir#b != iir#g) && (iir#b != iir#h) && (iir#b#data != iir#c#data) && (iir#b#data != iir#d#data) && (iir#b#data != iir#e#data) && (iir#b#data != iir#f#data) && (iir#b#data != iir#g#data) && (iir#b#data != iir#h#data) && (iir#c != iir#d) && (iir#c != iir#e) && (iir#c != iir#f) && (iir#c != iir#g) && (iir#c != iir#h) && (iir#c#data != iir#d#data) && (iir#c#data != iir#e#data) && (iir#c#data != iir#f#data) && (iir#c#data != iir#g#data) && (iir#c#data != iir#h#data) && (iir#d != iir#e) && (iir#d != iir#f) && (iir#d != iir#g) && (iir#d != iir#h) && (iir#d#data != iir#e#data) && (iir#d#data != iir#f#data) && (iir#d#data != iir#g#data) && (iir#d#data != iir#h#data) && (iir#e != iir#f) && (iir#e != iir#g) && (iir#e != iir#h) && (iir#e#data != iir#f#data) && (iir#e#data != iir#g#data) && (iir#e#data != iir#h#data) && (iir#f != iir#g) && (iir#f != iir#h) && (iir#f#data != iir#g#data) && (iir#f#data != iir#h#data) && (iir#g != iir#h) && (iir#g#data != iir#h#data);
+  assume (iir#a != iir#b) && (iir#a != iir#c) && (iir#a != iir#d) && (iir#a != iir#e) && (iir#a != iir#f) && (iir#a != iir#g) && (iir#a != iir#h) && (iir#b != iir#c) && (iir#b != iir#d) && (iir#b != iir#e) && (iir#b != iir#f) && (iir#b != iir#g) && (iir#b != iir#h) && (iir#c != iir#d) && (iir#c != iir#e) && (iir#c != iir#f) && (iir#c != iir#g) && (iir#c != iir#h) && (iir#d != iir#e) && (iir#d != iir#f) && (iir#d != iir#g) && (iir#d != iir#h) && (iir#e != iir#f) && (iir#e != iir#g) && (iir#e != iir#h) && (iir#f != iir#g) && (iir#f != iir#h) && (iir#g != iir#h);
   assume 0 <= I[iir#a];
   assume I[iir#a] <= R[iir#a];
   assume R[iir#a] <= C[iir#a];
@@ -832,70 +790,70 @@ procedure iir##rshift#anon$4#14()
   assume I[iir#c] == I[iir#f];
   assume I[iir#d] == I[iir#g];
   assume I[iir#h] == I[iir#g];
-  assume M[iir#f][0][data#int] == 0;
+  assume M[iir#f][0] == 0;
   assume R[iir#e] == (C[iir#f] - 1);
   assume (forall idx$: int :: 
-    (1 <= idx$) && (idx$ < C[iir#f]) ==> (M[iir#f][idx$][data#int] == M[iir#e][idx$ - 1][data#int])
+    (1 <= idx$) && (idx$ < C[iir#f]) ==> (M[iir#f][idx$] == M[iir#e][idx$ - 1])
   );
   assume R[iir#a] == C[iir#b];
   assume (forall idx$: int :: 
-    (0 <= idx$) && (idx$ < C[iir#b]) ==> (M[iir#b][idx$][data#int] == (85 * M[iir#a][idx$][data#int]))
+    (0 <= idx$) && (idx$ < C[iir#b]) ==> (M[iir#b][idx$] == (85 * M[iir#a][idx$]))
   );
   assume R[iir#d] == C[iir#e];
   assume (forall idx$: int :: 
-    (0 <= idx$) && (idx$ < C[iir#e]) ==> (M[iir#e][idx$][data#int] == (171 * M[iir#d][idx$][data#int]))
+    (0 <= idx$) && (idx$ < C[iir#e]) ==> (M[iir#e][idx$] == (171 * M[iir#d][idx$]))
   );
   assume R[iir#c] == C[iir#g];
   assume (forall idx$: int :: 
-    (0 <= idx$) && (idx$ < C[iir#g]) ==> (M[iir#g][idx$][data#int] == AT#RShift(M[iir#c][idx$][data#int], 8))
+    (0 <= idx$) && (idx$ < C[iir#g]) ==> (M[iir#g][idx$] == AT#RShift(M[iir#c][idx$], 8))
   );
   assume R[iir#b] == C[iir#c];
   assume R[iir#f] == C[iir#c];
   assume (forall idx$: int :: 
-    (0 <= idx$) && (idx$ < C[iir#c]) ==> (M[iir#c][idx$][data#int] == (M[iir#b][idx$][data#int] + M[iir#f][idx$][data#int]))
+    (0 <= idx$) && (idx$ < C[iir#c]) ==> (M[iir#c][idx$] == (M[iir#b][idx$] + M[iir#f][idx$]))
   );
   assume R[iir#g] == C[iir#d];
   assume R[iir#g] == C[iir#h];
   assume (forall idx$: int :: 
-    (0 <= idx$) && (idx$ < C[iir#d]) ==> (M[iir#d][idx$][data#int] == M[iir#g][idx$][data#int])
+    (0 <= idx$) && (idx$ < C[iir#d]) ==> (M[iir#d][idx$] == M[iir#g][idx$])
   );
   assume (forall idx$: int :: 
-    (0 <= idx$) && (idx$ < C[iir#h]) ==> (M[iir#h][idx$][data#int] == M[iir#g][idx$][data#int])
+    (0 <= idx$) && (idx$ < C[iir#h]) ==> (M[iir#h][idx$] == M[iir#g][idx$])
   );
   assume 1 <= (C[iir#c] - R[iir#c]);
-  in#i := M[iir#c][R[iir#c]][data#int];
+  in#i := M[iir#c][R[iir#c]];
   R[iir#c] := R[iir#c] + 1;
-  M[iir#g][C[iir#g]][data#int] := AT#RShift(in#i, 8);
+  M[iir#g][C[iir#g]] := AT#RShift(in#i, 8);
   C[iir#g] := C[iir#g] + 1;
-  assume M[iir#f][0][data#int] == 0;
+  assume M[iir#f][0] == 0;
   assume R[iir#e] == (C[iir#f] - 1);
   assume (forall idx$: int :: 
-    (1 <= idx$) && (idx$ < C[iir#f]) ==> (M[iir#f][idx$][data#int] == M[iir#e][idx$ - 1][data#int])
+    (1 <= idx$) && (idx$ < C[iir#f]) ==> (M[iir#f][idx$] == M[iir#e][idx$ - 1])
   );
   assume R[iir#a] == C[iir#b];
   assume (forall idx$: int :: 
-    (0 <= idx$) && (idx$ < C[iir#b]) ==> (M[iir#b][idx$][data#int] == (85 * M[iir#a][idx$][data#int]))
+    (0 <= idx$) && (idx$ < C[iir#b]) ==> (M[iir#b][idx$] == (85 * M[iir#a][idx$]))
   );
   assume R[iir#d] == C[iir#e];
   assume (forall idx$: int :: 
-    (0 <= idx$) && (idx$ < C[iir#e]) ==> (M[iir#e][idx$][data#int] == (171 * M[iir#d][idx$][data#int]))
+    (0 <= idx$) && (idx$ < C[iir#e]) ==> (M[iir#e][idx$] == (171 * M[iir#d][idx$]))
   );
   assume R[iir#c] == C[iir#g];
   assume (forall idx$: int :: 
-    (0 <= idx$) && (idx$ < C[iir#g]) ==> (M[iir#g][idx$][data#int] == AT#RShift(M[iir#c][idx$][data#int], 8))
+    (0 <= idx$) && (idx$ < C[iir#g]) ==> (M[iir#g][idx$] == AT#RShift(M[iir#c][idx$], 8))
   );
   assume R[iir#b] == C[iir#c];
   assume R[iir#f] == C[iir#c];
   assume (forall idx$: int :: 
-    (0 <= idx$) && (idx$ < C[iir#c]) ==> (M[iir#c][idx$][data#int] == (M[iir#b][idx$][data#int] + M[iir#f][idx$][data#int]))
+    (0 <= idx$) && (idx$ < C[iir#c]) ==> (M[iir#c][idx$] == (M[iir#b][idx$] + M[iir#f][idx$]))
   );
   assume R[iir#g] == C[iir#d];
   assume R[iir#g] == C[iir#h];
   assume (forall idx$: int :: 
-    (0 <= idx$) && (idx$ < C[iir#d]) ==> (M[iir#d][idx$][data#int] == M[iir#g][idx$][data#int])
+    (0 <= idx$) && (idx$ < C[iir#d]) ==> (M[iir#d][idx$] == M[iir#g][idx$])
   );
   assume (forall idx$: int :: 
-    (0 <= idx$) && (idx$ < C[iir#h]) ==> (M[iir#h][idx$][data#int] == M[iir#g][idx$][data#int])
+    (0 <= idx$) && (idx$ < C[iir#h]) ==> (M[iir#h][idx$] == M[iir#g][idx$])
   );
   assert {:msg "Action at 16.3 ('anon$4') for actor instance 'rsh1' might not preserve the channel invariant (#68)"} I[iir#f] == I[iir#e];
   assert {:msg "Action at 16.3 ('anon$4') for actor instance 'rsh1' might not preserve the channel invariant (#69)"} I[iir#b] == I[iir#a];
@@ -907,7 +865,7 @@ procedure iir##rshift#anon$4#14()
   assert {:msg "Action at 16.3 ('anon$4') for actor instance 'rsh1' might not preserve the channel invariant (#75)"} I[iir#h] == I[iir#g];
 }
 procedure iir##add#anon$0#15()
-  modifies C, R, M, I;
+  modifies C, R, M, I, H;
 {
   var iir#del1: Actor;
   var iir#mul1: Actor;
@@ -915,26 +873,18 @@ procedure iir##add#anon$0#15()
   var iir#rsh1: Actor;
   var iir#add1: Actor;
   var iir#spl1: Actor;
-  var iir#a: Chan;
-  var iir#a#data: Field (int);
-  var iir#b: Chan;
-  var iir#b#data: Field (int);
-  var iir#c: Chan;
-  var iir#c#data: Field (int);
-  var iir#d: Chan;
-  var iir#d#data: Field (int);
-  var iir#e: Chan;
-  var iir#e#data: Field (int);
-  var iir#f: Chan;
-  var iir#f#data: Field (int);
-  var iir#g: Chan;
-  var iir#g#data: Field (int);
-  var iir#h: Chan;
-  var iir#h#data: Field (int);
+  var iir#a: Chan (int);
+  var iir#b: Chan (int);
+  var iir#c: Chan (int);
+  var iir#d: Chan (int);
+  var iir#e: Chan (int);
+  var iir#f: Chan (int);
+  var iir#g: Chan (int);
+  var iir#h: Chan (int);
   var in1#i: int;
   var in2#j: int;
   assume (iir#del1 != iir#mul1) && (iir#del1 != iir#mul2) && (iir#del1 != iir#rsh1) && (iir#del1 != iir#add1) && (iir#del1 != iir#spl1) && (iir#mul1 != iir#mul2) && (iir#mul1 != iir#rsh1) && (iir#mul1 != iir#add1) && (iir#mul1 != iir#spl1) && (iir#mul2 != iir#rsh1) && (iir#mul2 != iir#add1) && (iir#mul2 != iir#spl1) && (iir#rsh1 != iir#add1) && (iir#rsh1 != iir#spl1) && (iir#add1 != iir#spl1);
-  assume (iir#a != iir#b) && (iir#a != iir#c) && (iir#a != iir#d) && (iir#a != iir#e) && (iir#a != iir#f) && (iir#a != iir#g) && (iir#a != iir#h) && (iir#a#data != iir#b#data) && (iir#a#data != iir#c#data) && (iir#a#data != iir#d#data) && (iir#a#data != iir#e#data) && (iir#a#data != iir#f#data) && (iir#a#data != iir#g#data) && (iir#a#data != iir#h#data) && (iir#b != iir#c) && (iir#b != iir#d) && (iir#b != iir#e) && (iir#b != iir#f) && (iir#b != iir#g) && (iir#b != iir#h) && (iir#b#data != iir#c#data) && (iir#b#data != iir#d#data) && (iir#b#data != iir#e#data) && (iir#b#data != iir#f#data) && (iir#b#data != iir#g#data) && (iir#b#data != iir#h#data) && (iir#c != iir#d) && (iir#c != iir#e) && (iir#c != iir#f) && (iir#c != iir#g) && (iir#c != iir#h) && (iir#c#data != iir#d#data) && (iir#c#data != iir#e#data) && (iir#c#data != iir#f#data) && (iir#c#data != iir#g#data) && (iir#c#data != iir#h#data) && (iir#d != iir#e) && (iir#d != iir#f) && (iir#d != iir#g) && (iir#d != iir#h) && (iir#d#data != iir#e#data) && (iir#d#data != iir#f#data) && (iir#d#data != iir#g#data) && (iir#d#data != iir#h#data) && (iir#e != iir#f) && (iir#e != iir#g) && (iir#e != iir#h) && (iir#e#data != iir#f#data) && (iir#e#data != iir#g#data) && (iir#e#data != iir#h#data) && (iir#f != iir#g) && (iir#f != iir#h) && (iir#f#data != iir#g#data) && (iir#f#data != iir#h#data) && (iir#g != iir#h) && (iir#g#data != iir#h#data);
+  assume (iir#a != iir#b) && (iir#a != iir#c) && (iir#a != iir#d) && (iir#a != iir#e) && (iir#a != iir#f) && (iir#a != iir#g) && (iir#a != iir#h) && (iir#b != iir#c) && (iir#b != iir#d) && (iir#b != iir#e) && (iir#b != iir#f) && (iir#b != iir#g) && (iir#b != iir#h) && (iir#c != iir#d) && (iir#c != iir#e) && (iir#c != iir#f) && (iir#c != iir#g) && (iir#c != iir#h) && (iir#d != iir#e) && (iir#d != iir#f) && (iir#d != iir#g) && (iir#d != iir#h) && (iir#e != iir#f) && (iir#e != iir#g) && (iir#e != iir#h) && (iir#f != iir#g) && (iir#f != iir#h) && (iir#g != iir#h);
   assume 0 <= I[iir#a];
   assume I[iir#a] <= R[iir#a];
   assume R[iir#a] <= C[iir#a];
@@ -968,72 +918,72 @@ procedure iir##add#anon$0#15()
   assume I[iir#c] == I[iir#f];
   assume I[iir#d] == I[iir#g];
   assume I[iir#h] == I[iir#g];
-  assume M[iir#f][0][data#int] == 0;
+  assume M[iir#f][0] == 0;
   assume R[iir#e] == (C[iir#f] - 1);
   assume (forall idx$: int :: 
-    (1 <= idx$) && (idx$ < C[iir#f]) ==> (M[iir#f][idx$][data#int] == M[iir#e][idx$ - 1][data#int])
+    (1 <= idx$) && (idx$ < C[iir#f]) ==> (M[iir#f][idx$] == M[iir#e][idx$ - 1])
   );
   assume R[iir#a] == C[iir#b];
   assume (forall idx$: int :: 
-    (0 <= idx$) && (idx$ < C[iir#b]) ==> (M[iir#b][idx$][data#int] == (85 * M[iir#a][idx$][data#int]))
+    (0 <= idx$) && (idx$ < C[iir#b]) ==> (M[iir#b][idx$] == (85 * M[iir#a][idx$]))
   );
   assume R[iir#d] == C[iir#e];
   assume (forall idx$: int :: 
-    (0 <= idx$) && (idx$ < C[iir#e]) ==> (M[iir#e][idx$][data#int] == (171 * M[iir#d][idx$][data#int]))
+    (0 <= idx$) && (idx$ < C[iir#e]) ==> (M[iir#e][idx$] == (171 * M[iir#d][idx$]))
   );
   assume R[iir#c] == C[iir#g];
   assume (forall idx$: int :: 
-    (0 <= idx$) && (idx$ < C[iir#g]) ==> (M[iir#g][idx$][data#int] == AT#RShift(M[iir#c][idx$][data#int], 8))
+    (0 <= idx$) && (idx$ < C[iir#g]) ==> (M[iir#g][idx$] == AT#RShift(M[iir#c][idx$], 8))
   );
   assume R[iir#b] == C[iir#c];
   assume R[iir#f] == C[iir#c];
   assume (forall idx$: int :: 
-    (0 <= idx$) && (idx$ < C[iir#c]) ==> (M[iir#c][idx$][data#int] == (M[iir#b][idx$][data#int] + M[iir#f][idx$][data#int]))
+    (0 <= idx$) && (idx$ < C[iir#c]) ==> (M[iir#c][idx$] == (M[iir#b][idx$] + M[iir#f][idx$]))
   );
   assume R[iir#g] == C[iir#d];
   assume R[iir#g] == C[iir#h];
   assume (forall idx$: int :: 
-    (0 <= idx$) && (idx$ < C[iir#d]) ==> (M[iir#d][idx$][data#int] == M[iir#g][idx$][data#int])
+    (0 <= idx$) && (idx$ < C[iir#d]) ==> (M[iir#d][idx$] == M[iir#g][idx$])
   );
   assume (forall idx$: int :: 
-    (0 <= idx$) && (idx$ < C[iir#h]) ==> (M[iir#h][idx$][data#int] == M[iir#g][idx$][data#int])
+    (0 <= idx$) && (idx$ < C[iir#h]) ==> (M[iir#h][idx$] == M[iir#g][idx$])
   );
   assume (1 <= (C[iir#b] - R[iir#b])) && (1 <= (C[iir#f] - R[iir#f]));
-  in1#i := M[iir#b][R[iir#b]][data#int];
+  in1#i := M[iir#b][R[iir#b]];
   R[iir#b] := R[iir#b] + 1;
-  in2#j := M[iir#f][R[iir#f]][data#int];
+  in2#j := M[iir#f][R[iir#f]];
   R[iir#f] := R[iir#f] + 1;
-  M[iir#c][C[iir#c]][data#int] := in1#i + in2#j;
+  M[iir#c][C[iir#c]] := in1#i + in2#j;
   C[iir#c] := C[iir#c] + 1;
-  assume M[iir#f][0][data#int] == 0;
+  assume M[iir#f][0] == 0;
   assume R[iir#e] == (C[iir#f] - 1);
   assume (forall idx$: int :: 
-    (1 <= idx$) && (idx$ < C[iir#f]) ==> (M[iir#f][idx$][data#int] == M[iir#e][idx$ - 1][data#int])
+    (1 <= idx$) && (idx$ < C[iir#f]) ==> (M[iir#f][idx$] == M[iir#e][idx$ - 1])
   );
   assume R[iir#a] == C[iir#b];
   assume (forall idx$: int :: 
-    (0 <= idx$) && (idx$ < C[iir#b]) ==> (M[iir#b][idx$][data#int] == (85 * M[iir#a][idx$][data#int]))
+    (0 <= idx$) && (idx$ < C[iir#b]) ==> (M[iir#b][idx$] == (85 * M[iir#a][idx$]))
   );
   assume R[iir#d] == C[iir#e];
   assume (forall idx$: int :: 
-    (0 <= idx$) && (idx$ < C[iir#e]) ==> (M[iir#e][idx$][data#int] == (171 * M[iir#d][idx$][data#int]))
+    (0 <= idx$) && (idx$ < C[iir#e]) ==> (M[iir#e][idx$] == (171 * M[iir#d][idx$]))
   );
   assume R[iir#c] == C[iir#g];
   assume (forall idx$: int :: 
-    (0 <= idx$) && (idx$ < C[iir#g]) ==> (M[iir#g][idx$][data#int] == AT#RShift(M[iir#c][idx$][data#int], 8))
+    (0 <= idx$) && (idx$ < C[iir#g]) ==> (M[iir#g][idx$] == AT#RShift(M[iir#c][idx$], 8))
   );
   assume R[iir#b] == C[iir#c];
   assume R[iir#f] == C[iir#c];
   assume (forall idx$: int :: 
-    (0 <= idx$) && (idx$ < C[iir#c]) ==> (M[iir#c][idx$][data#int] == (M[iir#b][idx$][data#int] + M[iir#f][idx$][data#int]))
+    (0 <= idx$) && (idx$ < C[iir#c]) ==> (M[iir#c][idx$] == (M[iir#b][idx$] + M[iir#f][idx$]))
   );
   assume R[iir#g] == C[iir#d];
   assume R[iir#g] == C[iir#h];
   assume (forall idx$: int :: 
-    (0 <= idx$) && (idx$ < C[iir#d]) ==> (M[iir#d][idx$][data#int] == M[iir#g][idx$][data#int])
+    (0 <= idx$) && (idx$ < C[iir#d]) ==> (M[iir#d][idx$] == M[iir#g][idx$])
   );
   assume (forall idx$: int :: 
-    (0 <= idx$) && (idx$ < C[iir#h]) ==> (M[iir#h][idx$][data#int] == M[iir#g][idx$][data#int])
+    (0 <= idx$) && (idx$ < C[iir#h]) ==> (M[iir#h][idx$] == M[iir#g][idx$])
   );
   assert {:msg "Action at 2.3 ('anon$0') for actor instance 'add1' might not preserve the channel invariant (#76)"} I[iir#f] == I[iir#e];
   assert {:msg "Action at 2.3 ('anon$0') for actor instance 'add1' might not preserve the channel invariant (#77)"} I[iir#b] == I[iir#a];
@@ -1045,7 +995,7 @@ procedure iir##add#anon$0#15()
   assert {:msg "Action at 2.3 ('anon$0') for actor instance 'add1' might not preserve the channel invariant (#83)"} I[iir#h] == I[iir#g];
 }
 procedure iir##split#anon$5#16()
-  modifies C, R, M, I;
+  modifies C, R, M, I, H;
 {
   var iir#del1: Actor;
   var iir#mul1: Actor;
@@ -1053,25 +1003,17 @@ procedure iir##split#anon$5#16()
   var iir#rsh1: Actor;
   var iir#add1: Actor;
   var iir#spl1: Actor;
-  var iir#a: Chan;
-  var iir#a#data: Field (int);
-  var iir#b: Chan;
-  var iir#b#data: Field (int);
-  var iir#c: Chan;
-  var iir#c#data: Field (int);
-  var iir#d: Chan;
-  var iir#d#data: Field (int);
-  var iir#e: Chan;
-  var iir#e#data: Field (int);
-  var iir#f: Chan;
-  var iir#f#data: Field (int);
-  var iir#g: Chan;
-  var iir#g#data: Field (int);
-  var iir#h: Chan;
-  var iir#h#data: Field (int);
+  var iir#a: Chan (int);
+  var iir#b: Chan (int);
+  var iir#c: Chan (int);
+  var iir#d: Chan (int);
+  var iir#e: Chan (int);
+  var iir#f: Chan (int);
+  var iir#g: Chan (int);
+  var iir#h: Chan (int);
   var in#i: int;
   assume (iir#del1 != iir#mul1) && (iir#del1 != iir#mul2) && (iir#del1 != iir#rsh1) && (iir#del1 != iir#add1) && (iir#del1 != iir#spl1) && (iir#mul1 != iir#mul2) && (iir#mul1 != iir#rsh1) && (iir#mul1 != iir#add1) && (iir#mul1 != iir#spl1) && (iir#mul2 != iir#rsh1) && (iir#mul2 != iir#add1) && (iir#mul2 != iir#spl1) && (iir#rsh1 != iir#add1) && (iir#rsh1 != iir#spl1) && (iir#add1 != iir#spl1);
-  assume (iir#a != iir#b) && (iir#a != iir#c) && (iir#a != iir#d) && (iir#a != iir#e) && (iir#a != iir#f) && (iir#a != iir#g) && (iir#a != iir#h) && (iir#a#data != iir#b#data) && (iir#a#data != iir#c#data) && (iir#a#data != iir#d#data) && (iir#a#data != iir#e#data) && (iir#a#data != iir#f#data) && (iir#a#data != iir#g#data) && (iir#a#data != iir#h#data) && (iir#b != iir#c) && (iir#b != iir#d) && (iir#b != iir#e) && (iir#b != iir#f) && (iir#b != iir#g) && (iir#b != iir#h) && (iir#b#data != iir#c#data) && (iir#b#data != iir#d#data) && (iir#b#data != iir#e#data) && (iir#b#data != iir#f#data) && (iir#b#data != iir#g#data) && (iir#b#data != iir#h#data) && (iir#c != iir#d) && (iir#c != iir#e) && (iir#c != iir#f) && (iir#c != iir#g) && (iir#c != iir#h) && (iir#c#data != iir#d#data) && (iir#c#data != iir#e#data) && (iir#c#data != iir#f#data) && (iir#c#data != iir#g#data) && (iir#c#data != iir#h#data) && (iir#d != iir#e) && (iir#d != iir#f) && (iir#d != iir#g) && (iir#d != iir#h) && (iir#d#data != iir#e#data) && (iir#d#data != iir#f#data) && (iir#d#data != iir#g#data) && (iir#d#data != iir#h#data) && (iir#e != iir#f) && (iir#e != iir#g) && (iir#e != iir#h) && (iir#e#data != iir#f#data) && (iir#e#data != iir#g#data) && (iir#e#data != iir#h#data) && (iir#f != iir#g) && (iir#f != iir#h) && (iir#f#data != iir#g#data) && (iir#f#data != iir#h#data) && (iir#g != iir#h) && (iir#g#data != iir#h#data);
+  assume (iir#a != iir#b) && (iir#a != iir#c) && (iir#a != iir#d) && (iir#a != iir#e) && (iir#a != iir#f) && (iir#a != iir#g) && (iir#a != iir#h) && (iir#b != iir#c) && (iir#b != iir#d) && (iir#b != iir#e) && (iir#b != iir#f) && (iir#b != iir#g) && (iir#b != iir#h) && (iir#c != iir#d) && (iir#c != iir#e) && (iir#c != iir#f) && (iir#c != iir#g) && (iir#c != iir#h) && (iir#d != iir#e) && (iir#d != iir#f) && (iir#d != iir#g) && (iir#d != iir#h) && (iir#e != iir#f) && (iir#e != iir#g) && (iir#e != iir#h) && (iir#f != iir#g) && (iir#f != iir#h) && (iir#g != iir#h);
   assume 0 <= I[iir#a];
   assume I[iir#a] <= R[iir#a];
   assume R[iir#a] <= C[iir#a];
@@ -1105,72 +1047,72 @@ procedure iir##split#anon$5#16()
   assume I[iir#c] == I[iir#f];
   assume I[iir#d] == I[iir#g];
   assume I[iir#h] == I[iir#g];
-  assume M[iir#f][0][data#int] == 0;
+  assume M[iir#f][0] == 0;
   assume R[iir#e] == (C[iir#f] - 1);
   assume (forall idx$: int :: 
-    (1 <= idx$) && (idx$ < C[iir#f]) ==> (M[iir#f][idx$][data#int] == M[iir#e][idx$ - 1][data#int])
+    (1 <= idx$) && (idx$ < C[iir#f]) ==> (M[iir#f][idx$] == M[iir#e][idx$ - 1])
   );
   assume R[iir#a] == C[iir#b];
   assume (forall idx$: int :: 
-    (0 <= idx$) && (idx$ < C[iir#b]) ==> (M[iir#b][idx$][data#int] == (85 * M[iir#a][idx$][data#int]))
+    (0 <= idx$) && (idx$ < C[iir#b]) ==> (M[iir#b][idx$] == (85 * M[iir#a][idx$]))
   );
   assume R[iir#d] == C[iir#e];
   assume (forall idx$: int :: 
-    (0 <= idx$) && (idx$ < C[iir#e]) ==> (M[iir#e][idx$][data#int] == (171 * M[iir#d][idx$][data#int]))
+    (0 <= idx$) && (idx$ < C[iir#e]) ==> (M[iir#e][idx$] == (171 * M[iir#d][idx$]))
   );
   assume R[iir#c] == C[iir#g];
   assume (forall idx$: int :: 
-    (0 <= idx$) && (idx$ < C[iir#g]) ==> (M[iir#g][idx$][data#int] == AT#RShift(M[iir#c][idx$][data#int], 8))
+    (0 <= idx$) && (idx$ < C[iir#g]) ==> (M[iir#g][idx$] == AT#RShift(M[iir#c][idx$], 8))
   );
   assume R[iir#b] == C[iir#c];
   assume R[iir#f] == C[iir#c];
   assume (forall idx$: int :: 
-    (0 <= idx$) && (idx$ < C[iir#c]) ==> (M[iir#c][idx$][data#int] == (M[iir#b][idx$][data#int] + M[iir#f][idx$][data#int]))
+    (0 <= idx$) && (idx$ < C[iir#c]) ==> (M[iir#c][idx$] == (M[iir#b][idx$] + M[iir#f][idx$]))
   );
   assume R[iir#g] == C[iir#d];
   assume R[iir#g] == C[iir#h];
   assume (forall idx$: int :: 
-    (0 <= idx$) && (idx$ < C[iir#d]) ==> (M[iir#d][idx$][data#int] == M[iir#g][idx$][data#int])
+    (0 <= idx$) && (idx$ < C[iir#d]) ==> (M[iir#d][idx$] == M[iir#g][idx$])
   );
   assume (forall idx$: int :: 
-    (0 <= idx$) && (idx$ < C[iir#h]) ==> (M[iir#h][idx$][data#int] == M[iir#g][idx$][data#int])
+    (0 <= idx$) && (idx$ < C[iir#h]) ==> (M[iir#h][idx$] == M[iir#g][idx$])
   );
   assume 1 <= (C[iir#g] - R[iir#g]);
-  in#i := M[iir#g][R[iir#g]][data#int];
+  in#i := M[iir#g][R[iir#g]];
   R[iir#g] := R[iir#g] + 1;
-  M[iir#d][C[iir#d]][data#int] := in#i;
+  M[iir#d][C[iir#d]] := in#i;
   C[iir#d] := C[iir#d] + 1;
-  M[iir#h][C[iir#h]][data#int] := in#i;
+  M[iir#h][C[iir#h]] := in#i;
   C[iir#h] := C[iir#h] + 1;
-  assume M[iir#f][0][data#int] == 0;
+  assume M[iir#f][0] == 0;
   assume R[iir#e] == (C[iir#f] - 1);
   assume (forall idx$: int :: 
-    (1 <= idx$) && (idx$ < C[iir#f]) ==> (M[iir#f][idx$][data#int] == M[iir#e][idx$ - 1][data#int])
+    (1 <= idx$) && (idx$ < C[iir#f]) ==> (M[iir#f][idx$] == M[iir#e][idx$ - 1])
   );
   assume R[iir#a] == C[iir#b];
   assume (forall idx$: int :: 
-    (0 <= idx$) && (idx$ < C[iir#b]) ==> (M[iir#b][idx$][data#int] == (85 * M[iir#a][idx$][data#int]))
+    (0 <= idx$) && (idx$ < C[iir#b]) ==> (M[iir#b][idx$] == (85 * M[iir#a][idx$]))
   );
   assume R[iir#d] == C[iir#e];
   assume (forall idx$: int :: 
-    (0 <= idx$) && (idx$ < C[iir#e]) ==> (M[iir#e][idx$][data#int] == (171 * M[iir#d][idx$][data#int]))
+    (0 <= idx$) && (idx$ < C[iir#e]) ==> (M[iir#e][idx$] == (171 * M[iir#d][idx$]))
   );
   assume R[iir#c] == C[iir#g];
   assume (forall idx$: int :: 
-    (0 <= idx$) && (idx$ < C[iir#g]) ==> (M[iir#g][idx$][data#int] == AT#RShift(M[iir#c][idx$][data#int], 8))
+    (0 <= idx$) && (idx$ < C[iir#g]) ==> (M[iir#g][idx$] == AT#RShift(M[iir#c][idx$], 8))
   );
   assume R[iir#b] == C[iir#c];
   assume R[iir#f] == C[iir#c];
   assume (forall idx$: int :: 
-    (0 <= idx$) && (idx$ < C[iir#c]) ==> (M[iir#c][idx$][data#int] == (M[iir#b][idx$][data#int] + M[iir#f][idx$][data#int]))
+    (0 <= idx$) && (idx$ < C[iir#c]) ==> (M[iir#c][idx$] == (M[iir#b][idx$] + M[iir#f][idx$]))
   );
   assume R[iir#g] == C[iir#d];
   assume R[iir#g] == C[iir#h];
   assume (forall idx$: int :: 
-    (0 <= idx$) && (idx$ < C[iir#d]) ==> (M[iir#d][idx$][data#int] == M[iir#g][idx$][data#int])
+    (0 <= idx$) && (idx$ < C[iir#d]) ==> (M[iir#d][idx$] == M[iir#g][idx$])
   );
   assume (forall idx$: int :: 
-    (0 <= idx$) && (idx$ < C[iir#h]) ==> (M[iir#h][idx$][data#int] == M[iir#g][idx$][data#int])
+    (0 <= idx$) && (idx$ < C[iir#h]) ==> (M[iir#h][idx$] == M[iir#g][idx$])
   );
   assert {:msg "Action at 20.3 ('anon$5') for actor instance 'spl1' might not preserve the channel invariant (#84)"} I[iir#f] == I[iir#e];
   assert {:msg "Action at 20.3 ('anon$5') for actor instance 'spl1' might not preserve the channel invariant (#85)"} I[iir#b] == I[iir#a];
@@ -1182,7 +1124,7 @@ procedure iir##split#anon$5#16()
   assert {:msg "Action at 20.3 ('anon$5') for actor instance 'spl1' might not preserve the channel invariant (#91)"} I[iir#h] == I[iir#g];
 }
 procedure iir#anon$6#input#in#17()
-  modifies C, R, M, I;
+  modifies C, R, M, I, H;
 {
   var iir#del1: Actor;
   var iir#mul1: Actor;
@@ -1190,24 +1132,16 @@ procedure iir#anon$6#input#in#17()
   var iir#rsh1: Actor;
   var iir#add1: Actor;
   var iir#spl1: Actor;
-  var iir#a: Chan;
-  var iir#a#data: Field (int);
-  var iir#b: Chan;
-  var iir#b#data: Field (int);
-  var iir#c: Chan;
-  var iir#c#data: Field (int);
-  var iir#d: Chan;
-  var iir#d#data: Field (int);
-  var iir#e: Chan;
-  var iir#e#data: Field (int);
-  var iir#f: Chan;
-  var iir#f#data: Field (int);
-  var iir#g: Chan;
-  var iir#g#data: Field (int);
-  var iir#h: Chan;
-  var iir#h#data: Field (int);
+  var iir#a: Chan (int);
+  var iir#b: Chan (int);
+  var iir#c: Chan (int);
+  var iir#d: Chan (int);
+  var iir#e: Chan (int);
+  var iir#f: Chan (int);
+  var iir#g: Chan (int);
+  var iir#h: Chan (int);
   assume (iir#del1 != iir#mul1) && (iir#del1 != iir#mul2) && (iir#del1 != iir#rsh1) && (iir#del1 != iir#add1) && (iir#del1 != iir#spl1) && (iir#mul1 != iir#mul2) && (iir#mul1 != iir#rsh1) && (iir#mul1 != iir#add1) && (iir#mul1 != iir#spl1) && (iir#mul2 != iir#rsh1) && (iir#mul2 != iir#add1) && (iir#mul2 != iir#spl1) && (iir#rsh1 != iir#add1) && (iir#rsh1 != iir#spl1) && (iir#add1 != iir#spl1);
-  assume (iir#a != iir#b) && (iir#a != iir#c) && (iir#a != iir#d) && (iir#a != iir#e) && (iir#a != iir#f) && (iir#a != iir#g) && (iir#a != iir#h) && (iir#a#data != iir#b#data) && (iir#a#data != iir#c#data) && (iir#a#data != iir#d#data) && (iir#a#data != iir#e#data) && (iir#a#data != iir#f#data) && (iir#a#data != iir#g#data) && (iir#a#data != iir#h#data) && (iir#b != iir#c) && (iir#b != iir#d) && (iir#b != iir#e) && (iir#b != iir#f) && (iir#b != iir#g) && (iir#b != iir#h) && (iir#b#data != iir#c#data) && (iir#b#data != iir#d#data) && (iir#b#data != iir#e#data) && (iir#b#data != iir#f#data) && (iir#b#data != iir#g#data) && (iir#b#data != iir#h#data) && (iir#c != iir#d) && (iir#c != iir#e) && (iir#c != iir#f) && (iir#c != iir#g) && (iir#c != iir#h) && (iir#c#data != iir#d#data) && (iir#c#data != iir#e#data) && (iir#c#data != iir#f#data) && (iir#c#data != iir#g#data) && (iir#c#data != iir#h#data) && (iir#d != iir#e) && (iir#d != iir#f) && (iir#d != iir#g) && (iir#d != iir#h) && (iir#d#data != iir#e#data) && (iir#d#data != iir#f#data) && (iir#d#data != iir#g#data) && (iir#d#data != iir#h#data) && (iir#e != iir#f) && (iir#e != iir#g) && (iir#e != iir#h) && (iir#e#data != iir#f#data) && (iir#e#data != iir#g#data) && (iir#e#data != iir#h#data) && (iir#f != iir#g) && (iir#f != iir#h) && (iir#f#data != iir#g#data) && (iir#f#data != iir#h#data) && (iir#g != iir#h) && (iir#g#data != iir#h#data);
+  assume (iir#a != iir#b) && (iir#a != iir#c) && (iir#a != iir#d) && (iir#a != iir#e) && (iir#a != iir#f) && (iir#a != iir#g) && (iir#a != iir#h) && (iir#b != iir#c) && (iir#b != iir#d) && (iir#b != iir#e) && (iir#b != iir#f) && (iir#b != iir#g) && (iir#b != iir#h) && (iir#c != iir#d) && (iir#c != iir#e) && (iir#c != iir#f) && (iir#c != iir#g) && (iir#c != iir#h) && (iir#d != iir#e) && (iir#d != iir#f) && (iir#d != iir#g) && (iir#d != iir#h) && (iir#e != iir#f) && (iir#e != iir#g) && (iir#e != iir#h) && (iir#f != iir#g) && (iir#f != iir#h) && (iir#g != iir#h);
   assume 0 <= I[iir#a];
   assume I[iir#a] <= R[iir#a];
   assume R[iir#a] <= C[iir#a];
@@ -1233,7 +1167,6 @@ procedure iir#anon$6#input#in#17()
   assume I[iir#h] <= R[iir#h];
   assume R[iir#h] <= C[iir#h];
   assume I[iir#h] == R[iir#h];
-  assume (C[iir#a] - I[iir#a]) < 1;
   assume I[iir#f] == I[iir#e];
   assume I[iir#b] == I[iir#a];
   assume I[iir#e] == I[iir#d];
@@ -1242,35 +1175,35 @@ procedure iir#anon$6#input#in#17()
   assume I[iir#c] == I[iir#f];
   assume I[iir#d] == I[iir#g];
   assume I[iir#h] == I[iir#g];
-  assume M[iir#f][0][data#int] == 0;
+  assume M[iir#f][0] == 0;
   assume R[iir#e] == (C[iir#f] - 1);
   assume (forall idx$: int :: 
-    (1 <= idx$) && (idx$ < C[iir#f]) ==> (M[iir#f][idx$][data#int] == M[iir#e][idx$ - 1][data#int])
+    (1 <= idx$) && (idx$ < C[iir#f]) ==> (M[iir#f][idx$] == M[iir#e][idx$ - 1])
   );
   assume R[iir#a] == C[iir#b];
   assume (forall idx$: int :: 
-    (0 <= idx$) && (idx$ < C[iir#b]) ==> (M[iir#b][idx$][data#int] == (85 * M[iir#a][idx$][data#int]))
+    (0 <= idx$) && (idx$ < C[iir#b]) ==> (M[iir#b][idx$] == (85 * M[iir#a][idx$]))
   );
   assume R[iir#d] == C[iir#e];
   assume (forall idx$: int :: 
-    (0 <= idx$) && (idx$ < C[iir#e]) ==> (M[iir#e][idx$][data#int] == (171 * M[iir#d][idx$][data#int]))
+    (0 <= idx$) && (idx$ < C[iir#e]) ==> (M[iir#e][idx$] == (171 * M[iir#d][idx$]))
   );
   assume R[iir#c] == C[iir#g];
   assume (forall idx$: int :: 
-    (0 <= idx$) && (idx$ < C[iir#g]) ==> (M[iir#g][idx$][data#int] == AT#RShift(M[iir#c][idx$][data#int], 8))
+    (0 <= idx$) && (idx$ < C[iir#g]) ==> (M[iir#g][idx$] == AT#RShift(M[iir#c][idx$], 8))
   );
   assume R[iir#b] == C[iir#c];
   assume R[iir#f] == C[iir#c];
   assume (forall idx$: int :: 
-    (0 <= idx$) && (idx$ < C[iir#c]) ==> (M[iir#c][idx$][data#int] == (M[iir#b][idx$][data#int] + M[iir#f][idx$][data#int]))
+    (0 <= idx$) && (idx$ < C[iir#c]) ==> (M[iir#c][idx$] == (M[iir#b][idx$] + M[iir#f][idx$]))
   );
   assume R[iir#g] == C[iir#d];
   assume R[iir#g] == C[iir#h];
   assume (forall idx$: int :: 
-    (0 <= idx$) && (idx$ < C[iir#d]) ==> (M[iir#d][idx$][data#int] == M[iir#g][idx$][data#int])
+    (0 <= idx$) && (idx$ < C[iir#d]) ==> (M[iir#d][idx$] == M[iir#g][idx$])
   );
   assume (forall idx$: int :: 
-    (0 <= idx$) && (idx$ < C[iir#h]) ==> (M[iir#h][idx$][data#int] == M[iir#g][idx$][data#int])
+    (0 <= idx$) && (idx$ < C[iir#h]) ==> (M[iir#h][idx$] == M[iir#g][idx$])
   );
   C[iir#a] := C[iir#a] + 1;
   assert {:msg "Channel invariant might be falsified by network input (#92)"} I[iir#f] == I[iir#e];
@@ -1283,7 +1216,7 @@ procedure iir#anon$6#input#in#17()
   assert {:msg "Channel invariant might be falsified by network input (#99)"} I[iir#h] == I[iir#g];
 }
 procedure iir#anon$6#exit#18()
-  modifies C, R, M, I;
+  modifies C, R, M, I, H;
 {
   var iir#del1: Actor;
   var iir#mul1: Actor;
@@ -1291,24 +1224,16 @@ procedure iir#anon$6#exit#18()
   var iir#rsh1: Actor;
   var iir#add1: Actor;
   var iir#spl1: Actor;
-  var iir#a: Chan;
-  var iir#a#data: Field (int);
-  var iir#b: Chan;
-  var iir#b#data: Field (int);
-  var iir#c: Chan;
-  var iir#c#data: Field (int);
-  var iir#d: Chan;
-  var iir#d#data: Field (int);
-  var iir#e: Chan;
-  var iir#e#data: Field (int);
-  var iir#f: Chan;
-  var iir#f#data: Field (int);
-  var iir#g: Chan;
-  var iir#g#data: Field (int);
-  var iir#h: Chan;
-  var iir#h#data: Field (int);
+  var iir#a: Chan (int);
+  var iir#b: Chan (int);
+  var iir#c: Chan (int);
+  var iir#d: Chan (int);
+  var iir#e: Chan (int);
+  var iir#f: Chan (int);
+  var iir#g: Chan (int);
+  var iir#h: Chan (int);
   assume (iir#del1 != iir#mul1) && (iir#del1 != iir#mul2) && (iir#del1 != iir#rsh1) && (iir#del1 != iir#add1) && (iir#del1 != iir#spl1) && (iir#mul1 != iir#mul2) && (iir#mul1 != iir#rsh1) && (iir#mul1 != iir#add1) && (iir#mul1 != iir#spl1) && (iir#mul2 != iir#rsh1) && (iir#mul2 != iir#add1) && (iir#mul2 != iir#spl1) && (iir#rsh1 != iir#add1) && (iir#rsh1 != iir#spl1) && (iir#add1 != iir#spl1);
-  assume (iir#a != iir#b) && (iir#a != iir#c) && (iir#a != iir#d) && (iir#a != iir#e) && (iir#a != iir#f) && (iir#a != iir#g) && (iir#a != iir#h) && (iir#a#data != iir#b#data) && (iir#a#data != iir#c#data) && (iir#a#data != iir#d#data) && (iir#a#data != iir#e#data) && (iir#a#data != iir#f#data) && (iir#a#data != iir#g#data) && (iir#a#data != iir#h#data) && (iir#b != iir#c) && (iir#b != iir#d) && (iir#b != iir#e) && (iir#b != iir#f) && (iir#b != iir#g) && (iir#b != iir#h) && (iir#b#data != iir#c#data) && (iir#b#data != iir#d#data) && (iir#b#data != iir#e#data) && (iir#b#data != iir#f#data) && (iir#b#data != iir#g#data) && (iir#b#data != iir#h#data) && (iir#c != iir#d) && (iir#c != iir#e) && (iir#c != iir#f) && (iir#c != iir#g) && (iir#c != iir#h) && (iir#c#data != iir#d#data) && (iir#c#data != iir#e#data) && (iir#c#data != iir#f#data) && (iir#c#data != iir#g#data) && (iir#c#data != iir#h#data) && (iir#d != iir#e) && (iir#d != iir#f) && (iir#d != iir#g) && (iir#d != iir#h) && (iir#d#data != iir#e#data) && (iir#d#data != iir#f#data) && (iir#d#data != iir#g#data) && (iir#d#data != iir#h#data) && (iir#e != iir#f) && (iir#e != iir#g) && (iir#e != iir#h) && (iir#e#data != iir#f#data) && (iir#e#data != iir#g#data) && (iir#e#data != iir#h#data) && (iir#f != iir#g) && (iir#f != iir#h) && (iir#f#data != iir#g#data) && (iir#f#data != iir#h#data) && (iir#g != iir#h) && (iir#g#data != iir#h#data);
+  assume (iir#a != iir#b) && (iir#a != iir#c) && (iir#a != iir#d) && (iir#a != iir#e) && (iir#a != iir#f) && (iir#a != iir#g) && (iir#a != iir#h) && (iir#b != iir#c) && (iir#b != iir#d) && (iir#b != iir#e) && (iir#b != iir#f) && (iir#b != iir#g) && (iir#b != iir#h) && (iir#c != iir#d) && (iir#c != iir#e) && (iir#c != iir#f) && (iir#c != iir#g) && (iir#c != iir#h) && (iir#d != iir#e) && (iir#d != iir#f) && (iir#d != iir#g) && (iir#d != iir#h) && (iir#e != iir#f) && (iir#e != iir#g) && (iir#e != iir#h) && (iir#f != iir#g) && (iir#f != iir#h) && (iir#g != iir#h);
   assume 0 <= I[iir#a];
   assume I[iir#a] <= R[iir#a];
   assume R[iir#a] <= C[iir#a];
@@ -1342,35 +1267,35 @@ procedure iir#anon$6#exit#18()
   assume I[iir#c] == I[iir#f];
   assume I[iir#d] == I[iir#g];
   assume I[iir#h] == I[iir#g];
-  assume M[iir#f][0][data#int] == 0;
+  assume M[iir#f][0] == 0;
   assume R[iir#e] == (C[iir#f] - 1);
   assume (forall idx$: int :: 
-    (1 <= idx$) && (idx$ < C[iir#f]) ==> (M[iir#f][idx$][data#int] == M[iir#e][idx$ - 1][data#int])
+    (1 <= idx$) && (idx$ < C[iir#f]) ==> (M[iir#f][idx$] == M[iir#e][idx$ - 1])
   );
   assume R[iir#a] == C[iir#b];
   assume (forall idx$: int :: 
-    (0 <= idx$) && (idx$ < C[iir#b]) ==> (M[iir#b][idx$][data#int] == (85 * M[iir#a][idx$][data#int]))
+    (0 <= idx$) && (idx$ < C[iir#b]) ==> (M[iir#b][idx$] == (85 * M[iir#a][idx$]))
   );
   assume R[iir#d] == C[iir#e];
   assume (forall idx$: int :: 
-    (0 <= idx$) && (idx$ < C[iir#e]) ==> (M[iir#e][idx$][data#int] == (171 * M[iir#d][idx$][data#int]))
+    (0 <= idx$) && (idx$ < C[iir#e]) ==> (M[iir#e][idx$] == (171 * M[iir#d][idx$]))
   );
   assume R[iir#c] == C[iir#g];
   assume (forall idx$: int :: 
-    (0 <= idx$) && (idx$ < C[iir#g]) ==> (M[iir#g][idx$][data#int] == AT#RShift(M[iir#c][idx$][data#int], 8))
+    (0 <= idx$) && (idx$ < C[iir#g]) ==> (M[iir#g][idx$] == AT#RShift(M[iir#c][idx$], 8))
   );
   assume R[iir#b] == C[iir#c];
   assume R[iir#f] == C[iir#c];
   assume (forall idx$: int :: 
-    (0 <= idx$) && (idx$ < C[iir#c]) ==> (M[iir#c][idx$][data#int] == (M[iir#b][idx$][data#int] + M[iir#f][idx$][data#int]))
+    (0 <= idx$) && (idx$ < C[iir#c]) ==> (M[iir#c][idx$] == (M[iir#b][idx$] + M[iir#f][idx$]))
   );
   assume R[iir#g] == C[iir#d];
   assume R[iir#g] == C[iir#h];
   assume (forall idx$: int :: 
-    (0 <= idx$) && (idx$ < C[iir#d]) ==> (M[iir#d][idx$][data#int] == M[iir#g][idx$][data#int])
+    (0 <= idx$) && (idx$ < C[iir#d]) ==> (M[iir#d][idx$] == M[iir#g][idx$])
   );
   assume (forall idx$: int :: 
-    (0 <= idx$) && (idx$ < C[iir#h]) ==> (M[iir#h][idx$][data#int] == M[iir#g][idx$][data#int])
+    (0 <= idx$) && (idx$ < C[iir#h]) ==> (M[iir#h][idx$] == M[iir#g][idx$])
   );
   assume (C[iir#a] - I[iir#a]) == 1;
   assume !(1 <= (C[iir#e] - R[iir#e]));
@@ -1379,8 +1304,8 @@ procedure iir#anon$6#exit#18()
   assume !(1 <= (C[iir#c] - R[iir#c]));
   assume !((1 <= (C[iir#b] - R[iir#b])) && (1 <= (C[iir#f] - R[iir#f])));
   assume !(1 <= (C[iir#g] - R[iir#g]));
-  assert {:msg "26.13: Network action postcondition might not hold (#100)"} M[iir#h][0][data#int] == AT#RShift(85 * M[iir#a][0][data#int], 8);
-  assert {:msg "27.13: Network action postcondition might not hold (#101)"} (0 < I[iir#h]) ==> (M[iir#h][I[iir#h]][data#int] == AT#RShift((171 * M[iir#h][I[iir#h] - 1][data#int]) + (85 * M[iir#a][I[iir#a]][data#int]), 8));
+  assert {:msg "26.13: Network action postcondition might not hold (#100)"} M[iir#h][0] == AT#RShift(85 * M[iir#a][0], 8);
+  assert {:msg "27.13: Network action postcondition might not hold (#101)"} (0 < I[iir#h]) ==> (M[iir#h][I[iir#h]] == AT#RShift((171 * M[iir#h][I[iir#h] - 1]) + (85 * M[iir#a][I[iir#a]]), 8));
   R[iir#h] := R[iir#h] + 1;
   I := R;
   assert {:msg "The network might not preserve the channel invariant (#102)"} I[iir#f] == I[iir#e];
