tests/ChSum.bpl
@@ -1,0 +1,71 @@
+// ---------------------------------------------------------------
+// -- Types and global variables ---------------------------------
+// ---------------------------------------------------------------
+type Ref;
+type Chan a;
+type Field a;
+type Actor;
+type CType = <a>[Chan a]int;
+type MType = <a>[Chan a][int]a;
+type Obj = <a>[Field a]a;
+type HType = [Ref]Obj;
+
+var M: MType;
+var C: CType;
+var R: CType;
+var I: CType;
+
+var H: HType;
+
+const unique this#: Actor;
+
+function AT#Min(x:int, y: int): int { if x <= y then x else y }
+
+function AT#ChSum(MType, Chan int, int): int;
+axiom (
+  forall mm: MType, ch: Chan int, limit: int :: {AT#ChSum(mm,ch,limit)} {AT#ChSum(mm,ch,limit-1)} 
+    (limit > 0 ==> AT#ChSum(mm,ch,limit) == mm[ch][limit-1]+AT#ChSum(mm,ch,limit-1)) &&
+    (limit == 0 ==> AT#ChSum(mm,ch,limit) == 0)
+);
+axiom (
+  forall mm: MType, ch: Chan int :: {AT#ChSum(mm,ch,0)} 
+    AT#ChSum(mm,ch,0) == 0
+);
+
+// ---------------------------------------------------------------
+// -- End of prelude ---------------------------------------------
+// ---------------------------------------------------------------
+
+procedure ChSum#init#0()
+  modifies C, R, M, I, H;
+{
+  var x: Chan (int);
+  var y: Chan (int);
+  var sum: int;
+  assume x != y;
+  assume R[x] == 0;
+  assume C[y] == 0;
+  sum := 0;
+  assert {:msg "3.13: Initialization might not establish the invariant (#0)"} R[x] == C[y];
+  assert {:msg "4.13: Initialization might not establish the invariant (#1)"} (C[y] > 0) ==> (M[y][C[y] - 1] == AT#ChSum(M, x, R[x]));
+}
+procedure ChSum#anon$1#1()
+  modifies C, R, M, I, H;
+{
+  var x: Chan (int);
+  var y: Chan (int);
+  var sum: int;
+  var x#0: int;
+  assume x != y;
+  assume 0 <= R[x];
+  assume 0 <= C[y];
+  assume R[x] == C[y];
+  assume (C[y] > 0) ==> (M[y][C[y] - 1] == AT#ChSum(M, x, R[x]));
+  x#0 := M[x][R[x]];
+  R[x] := R[x] + 1;
+  sum := sum + x#0;
+  M[y][C[y]] := sum;
+  C[y] := C[y] + 1;
+  assert {:msg "3.13: Action at 11.3 might not preserve invariant (#2)"} R[x] == C[y];
+  assert {:msg "4.13: Action at 11.3 might not preserve invariant (#3)"} (C[y] > 0) ==> (M[y][C[y] - 1] == AT#ChSum(M, x, R[x]));
+}
