tests/List.bpl
@@ -1,0 +1,75 @@
+// ---------------------------------------------------------------
+// -- Types and global variables ---------------------------------
+// ---------------------------------------------------------------
+type Ref;
+type Chan a;
+type Field a;
+type Actor;
+type CType = <a>[Chan a]int;
+type MType = <a>[Chan a][int]a;
+type Obj = <a>[Field a]a;
+type HType = [Ref]Obj;
+
+var M: MType;
+var C: CType;
+var R: CType;
+var I: CType;
+
+var H: HType;
+
+const unique this#: Actor;
+
+function AT#Min(x:int, y: int): int { if x <= y then x else y }
+
+// ---------------------------------------------------------------
+// -- Axiomatisation for map data type ---------------------------
+// ---------------------------------------------------------------
+type Map a b;
+
+function Map#Select<T,U>(Map T U, T): U;
+function Map#Store<T,U>(Map T U, T, U): Map T U;
+axiom (
+  forall<T,U> m: Map T U, k1: T, val: U :: { Map#Store(m,k1,val) }
+    Map#Select(Map#Store(m,k1,val),k1) == val
+);
+axiom (
+  forall<T,U> m: Map T U, k1: T, k2: T, val: U :: { Map#Select(Map#Store(m,k1,val),k2) }
+    k1 != k2 ==> Map#Select(Map#Store(m,k1,val),k2) == Map#Select(m,k2)
+);
+
+// ---------------------------------------------------------------
+// -- End of prelude ---------------------------------------------
+// ---------------------------------------------------------------
+
+procedure List1#init#0()
+  modifies C, R, M, I, H;
+{
+  var x: Chan (int);
+  var y: Chan (int);
+  var test: Map (int) (int);
+  assume x != y;
+  assume R[x] == 0;
+  assume C[y] == 0;
+  test := Map#Store(test, 0, 0);
+  test := Map#Store(test, 1, 1);
+  assert {:msg "5.12: Initialization might not establish the invariant (#0)"} (Map#Select(test, 0) == 0) && (Map#Select(test, 1) == 1);
+}
+procedure List1#anon$1#1()
+  modifies C, R, M, I, H;
+{
+  var x: Chan (int);
+  var y: Chan (int);
+  var test: Map (int) (int);
+  var x#0: int;
+  assume x != y;
+  assume 0 <= R[x];
+  assume 0 <= C[y];
+  assume (Map#Select(test, 0) == 0) && (Map#Select(test, 1) == 1);
+  x#0 := M[x][R[x]];
+  R[x] := R[x] + 1;
+  test := Map#Store(test, 0, 0);
+  test := Map#Store(test, 1, 1);
+  M[y][C[y]] := x#0;
+  C[y] := C[y] + 1;
+  assert {:msg "5.12: Action at 13.2 might not preserve invariant (#1)"} (Map#Select(test, 0) == 0) && (Map#Select(test, 1) == 1);
+}
